#+TITLE: 2 Wave and Oscillation Homework
#+AUTHOR: 2024110144 陈有骏
#+LATEX_COMPILER: xelatex
#+LATEX_CLASS: article
#+LATEX_CLASS_OPTIONS: [a4paper,10pt]
#+LATEX_HEADER: \usepackage[margin=0.5in]{geometry}
#+LATEX_HEADER: \usepackage{xeCJK}
#+LATEX_HEADER: \usepackage{fontspec}
#+LATEX_HEADER: \setCJKmainfont{WenQuanYi Zen Hei}
#+OPTIONS: \n:t toc:nil num:nil date:nil

first the normal ones,
later change the cosine stuff to get 2 other expressions.

the $x$ expressions are $x=A\cos (\omega t+\phi)$, $x=Ae^{-\beta t}\cos (\omega_d t+\phi)$ and $x=A\cos (\omega t - \delta)$ respectively
so after differencing them
we get $v=-A\omega \sin (\omega t+\phi)$ for simple harmonic motion
$$\begin{aligned}
v &= A (-\omega_d e^{-\beta t} \sin (\omega_d t + \phi)- \beta e^{-\beta t} \cos (\omega_d t+\phi)\\
&= -Ae^{-\beta t} (\omega_d \sin (\omega_d t + \phi) + \beta \cos (\omega_d t+\phi))
\end{aligned}$$
for dumping variation
for forced harmonic motion, $v = -A \omega \sin (\omega t - \delta)$
after differencing again
we get $a=-A\omega^2 \cos (\omega t+\phi)$
$$\begin{aligned}
a &= A\beta e^{-\beta t} (\omega_d \sin (\omega_d t + \phi) + \beta \cos (\omega_d t+\phi))\\
&\quad - Ae^{-\beta t} (\omega_d^2 \cos (\omega_d t + \phi) - \beta \omega_d \sin (\omega_d t+\phi))\\
&= Ae^{-\beta t} (2\beta\omega_d \sin (\omega_d t + \phi) + (\beta^2-\omega_d^2) \cos (\omega_d t + \phi))
\end{aligned}$$
and $a=-A\omega^2 \cos (\omega t - \delta)$ respectively

for the other 2 expressions, we shall use sine and cosine exchange rules and Euler's $e^{i\theta}=\cos\theta+i\sin\theta$
since sine and cosine just requires the change of symbol and adding $+\frac{\pi}{2}$, I would like to skip these
specially, for that variation with Euler's equation,
$$\begin{aligned}
x &= \frac{1}{2} A \left(e^{i(\omega t + \phi)}+e^{-i(\omega t + \phi)}\right)\\
x &= \frac{1}{2} A e^{-\beta t} \left(e^{i(\omega_d t + \phi)}+e^{-i(\omega_d t + \phi)}\right)\\
x &= \frac{1}{2} A \left(e^{i(\omega t - \delta)}+e^{-i(\omega t - \delta)}\right)
\end{aligned}$$
then
$$\begin{aligned}
v &= \frac{1}{2} iA \omega \left(e^{i(\omega t + \phi)}-e^{-i(\omega t + \phi)}\right)\\
v &= -\frac{1}{2} A e^{-\beta t} \left(\beta \left(e^{i(\omega_d t + \phi)}+e^{-i(\omega_d t + \phi)}\right) + i\omega_d \left(e^{i(\omega t + \phi)}-e^{-i(\omega t + \phi)}\right)\right)\\
v &= \frac{1}{2} iA \omega \left(e^{i(\omega t - \delta)}-e^{-i(\omega t - \delta)}\right)
\end{aligned}$$
and
$$\begin{aligned}
a &= -\frac{1}{2} A \omega^2 \left(e^{i(\omega t + \phi)}+e^{-i(\omega t + \phi)}\right)\\
a &= \frac{1}{2} A e^{-\beta t} \left((\beta^2-\omega_d^2+\beta \omega_d)e^{i(\omega_d t + \phi)}+(\beta^2-\omega_d^2-\beta \omega_d)e^{-i(\omega_d t + \phi)}\right)\\
a &= -\frac{1}{2} A \omega^2 \left(e^{i(\omega t - \delta)}+e^{-i(\omega t - \delta)}\right)
\end{aligned}$$
respectively
