#+TITLE: Week 4.27 Math Homework
#+AUTHOR: 2024110144 陈有骏
#+LATEX_COMPILER: xelatex
#+LATEX_CLASS: article
#+LATEX_CLASS_OPTIONS: [a4paper,10pt]
#+LATEX_HEADER: \usepackage[margin=0.5in]{geometry}
#+LATEX_HEADER: \usepackage{xeCJK}
#+OPTIONS: \n:t toc:nil num:nil date:nil

#+begin_comment
4.27 Thomas 16.1 1-46 mod 6
left: 24 42 (both failed to integrate)
4.28 Thomas 16.2 1-60 mod 6
left: 36 42 48 54 60
#+end_comment

* 4.27
** 6
the answer is $b$
because firstly, the graph should be a straight line
secondarily, the graph should be only in $yz$ plain
** 12
$$r(t)=(4\cos t)\vec{i} + (4\sin t)\vec{j} + 3t\vec{k}$$
$$r'(t)=-4\sin t \vec{i} + 4\cos t \vec{j} +3\vec{k}$$
$$||r'(t)||=5$$
$$-2\pi\leq t \leq 2\pi$$
$$\begin{align*}
\int_C \sqrt{x^2+y^2} ds
&= 5 \int_C \sqrt{x^2+y^2} dt\\
&= 5 \int_C 4 dt\\
&= 20 \int_C dt\\
&= 20 \times 4\pi\\
&= 80\pi
\end{align*}$$
** 18
we can see that $x$ is $0$ on the circle
so we just need to calculate with $x=0$
$$\int_C -\sqrt{x^2+z^2} ds
&= -\int_C \sqrt{z^2} ds\\
&= -a\int_C a |\sin t| dt\\
&= -a\int_0^{2\pi} a |\sin t| dt\\
&= -a^2\int_0^{2\pi} |\sin t| dt\\
&= -2a^2\int_0^{\pi} \sin t dt\\
&= -2a^2 \cos t |_0^{\pi}\\
&= -2a^2 \times (-2)\\
&= 4a^2
\end{align*}$$
** 24
$$r'(t)=3t^2\vec{i}+4t^3\vec{j}$$
$$||r'(t)||=\sqrt{9t^4+16t^9}$$
$$\begin{align*}
\int_C \frac{\sqrt{y}}{x} ds
&= \int_C \frac{1}{t} \cdot \sqrt{9t^4+16t^9} dt\\
&= \int_C \sqrt{9t^2+16t^7} dt\\
&= \int_C t \cdot \sqrt{9+16t^5} dt\\
&= \frac{1}{2} \int_C \sqrt{9+16t^5} dt^2\\
&= \frac{1}{2} \int_{\frac{1}{2}}^1 \sqrt{9+16t^5} dt^2\\
&= \frac{1}{2} \int_{\frac{1}{4}}^1 \sqrt{9+16t^{2.5}} dt
\end{align*}$$
no idea how to integrate this
** 30
$$r(t)=2\cos t \vec{i} + 2\sin t \vec{j}$$
t range: $[0,\frac{\pi}{2}]$
$$r'(t)=-2\sin t \vec{i} + 2\cos t \vec{j}$$
$$||r'(t)||=2$$
$$\begin{align*}
\int_C (x^2-y) ds
&= \int_C (4\cos^2 t - 2\sin t) \cdot 2 dt\\
&= 4\int_C (2\cos^2 t - \sin t) dt\\
&= 4\int_0^{\frac{\pi}{2}} (2\cos^2 t - \sin t) dt\\
&= 8\int_0^{\frac{\pi}{2}} \cos^2 t dt + 4\cos t |_0^{\frac{\pi}{2}}\\
&= 8\int_0^{\frac{\pi}{2}} \cos^2 t dt - 4\\
&= 8\int_0^{\frac{\pi}{2}} \frac{1+\cos 2t}{2} dt - 4\\
&= 4\int_0^{\frac{\pi}{2}} \frac{1+\cos 2t}{2} d2t - 4\\
&= 4\int_0^{\pi} \frac{1+\cos t}{2} dt - 4\\
&= 2(t+\sin t |_0^{\pi}) - 4\\
&= 2\pi - 4
\end{align*}$$
** 36
$$r'(t)=\vec{i}+2\vec{j}+\sqrt{t}\vec{k}$$
$$||r'(t)||=\sqrt{5+t}$$
$$\begin{align*}
\int_0^2 3\times (5+t) dt
&= 3\int_0^2 5+t dt\\
&= 3 (5t+\frac{t^2}{2} |_0^2)\\
&= 3 (10+2)\\
&= 36
\end{align*}$$
** 42
$$r(t)=t\vec{i}+\frac{2\sqrt{2}}{3}t^{\frac{3}{2}}\vec{j}+\frac{t^2}{2}\vec{k}$$
$$r'(t)=\vec{i}+\sqrt{2t}\vec{j}+t\vec{k}$$
$$||r'(t)||=\sqrt{1+5t^2}$$
$$\begin{align*}
M
&= \int_0^2 \frac{\sqrt{1+5t^2}}{t+1} dt\\
&= \int_1^3 \frac{\sqrt{1+5(t-1)^2}}{t} dt\\
&= \int_1^3 \frac{\sqrt{1+5(t^2-2t+1)}}{t} dt\\
&= \int_1^3 \frac{\sqrt{5t^2-10t+6}}{t} dt\\
&= \int_1^3 \sqrt{5-\frac{10}{t}+\frac{6}{t^2}} dt
\end{align*}$$
well, again failed to integrate this
the step left is to calculate $\int_0^2 \frac{\sqrt{1+5t^2}}{t+1} x dt$
and $\int_0^2 \frac{\sqrt{1+5t^2}}{t+1} y dt$
then divide with $x$,$y$ respectively

* 4.28
** 6
at $(0,0)$, $F=\vec{0}$
at $(a,b)$ where $a,b$ won't be $0$ at the same time
$F=(a+b,b-a)-(a,b)$
so $F=(b,-a)$
then $F=b\vec{i}-a\vec{j}$
** 12
$$\vec{F}=(y+z)\vec{i}+(x+z)\vec{j}+(x+y)\vec{k}$$
*** a
$$\frac{dr}{dt}=\vec{i}+\vec{j}+\vec{k}$$
$$\begin{align*}
\int_{C_1} \vec{F} dr
&= \int_{C_1} \vec{F} \cdot \frac{dr}{dt} dt\\
&= \int_{C_1} \vec{F} \cdot (\vec{i}+\vec{j}+\vec{k}) dt\\
&= \int_{C_1} \left((y+z)\vec{i}+(x+z)\vec{j}+(x+y)\vec{k}\right) \cdot (\vec{i}+\vec{j}+\vec{k}) dt\\
&= \int_0^1 \left((y+z)\vec{i}+(x+z)\vec{j}+(x+y)\vec{k}\right) \cdot (\vec{i}+\vec{j}+\vec{k}) dt\\
&= \int_0^1 \left((y+z)+(x+z)+(x+y)\right) dt\\
&= \int_0^1 6t dt\\
&= 3 t^2 |_0^1\\
&= 3
\end{align*}$$
*** b
$$\frac{dr}{dt}=\vec{i}+2t\vec{j}+4t^3\vec{k}$$
$$\begin{align*}
\int_{C_1} \vec{F} dr
&= \int_{C_1} \vec{F} \cdot \frac{dr}{dt} dt\\
&= \int_{C_1} \vec{F} \cdot (\vec{i}+2t\vec{j}+4t^3\vec{k}) dt\\
&= \int_0^1 \vec{F} \cdot (\vec{i}+2t\vec{j}+4t^3\vec{k}) dt\\
&= \int_0^1 ((y+z)\vec{i}+(x+z)\vec{j}+(x+y)\vec{k}) \cdot (\vec{i}+2t\vec{j}+4t^3\vec{k}) dt\\
&= \int_0^1 ((y+z)+2t(x+z)+4t^3(x+y)) dt\\
&= \int_0^1 (2t+4t^2+8t^4) dt\\
&= (t^2+\frac{4t^3}{3}+\frac{8t^5}{5})|_0^1\\
&= 1+\frac{4}{3}+\frac{8}{5}\\
&= \frac{7}{3}+\frac{8}{5}\\
&= \frac{35}{15}+\frac{24}{15}\\
&= \frac{59}{15}
\end{align*}$$
*** c
$$C_3:\, r_3 (t)=t\vec{i}+t\vec{j}$$
$$C_4:\, r_4 (t)=t\vec{k}$$
$$\frac{dr_3}{dt}=\vec{i}+\vec{j}$$
$$\frac{dr_4}{dt}=\vec{k}$$
$$\begin{align*}
\int_{C_3 \cup C_4} \vec{F} dr
&= \int_{C_3} \vec{F} dr_3 + \int_{C_4} \vec{F} dr_4\\
&= \int_{C_3} ((y+z)\vec{i}+(x+z)\vec{j}+(x+y)\vec{k}) dr_3 + \int_{C_4} ((y+z)\vec{i}+(x+z)\vec{j}+(x+y)\vec{k}) dr_4\\
&= \int_{C_3} ((y+z)+(x+z)) dt + \int_{C_4} (x+y) dt\\
&= \int_0^1 ((y+z)+(x+z)) dt + \int_0^1 (x+y) dt\\
&= \int_0^1 (y+x) dt + \int_0^1 2 dt\\
&= \int_0^1 2t dt + \int_0^1 2 dt\\
&= t^2 |_0^1 + 2t |_0^1\\
&= 1 + 2\\
&= 3
\end{align*}$$
** 18
$$r(t)=(\cos t)\vec{i}+(\sin t)\vec{j}-(\cos t)\vec{k},\,0\leq t\leq \pi$$
$$r'(t)=-\sin t \vec{i} + \cos t \vec{j} + \sin t \vec{k}$$
*** a
$$\begin{align*}
\int_C xz dx
&= \int_C xz \cdot \frac{dx}{dt} dt\\
&= \int_0^{\pi} -\cos^2 t \cdot -\sin t dt\\
&= \int_0^{\pi} \cos^2 t \sin t dt\\
&= -\int_0^{\pi} \cos^2 t d\cos t\\
&= -\int_1^{-1} t^2 dt\\
&= \int_{-1}^1 t^2 dt\\
&= \frac{t^3}{3}|_{-1}^1\\
&= \frac{2}{3}
\end{align*}$$
*** b
$$\begin{align*}
\int_C xz dy
&= \int_C xz \cdot \frac{dy}{dt} dt\\
&= \int_0^{\pi} -\cos^2 t \cdot \cos t dt\\
&= -\int_0^{\pi} \cos^3 t dt\\
&= -\int_0^{\pi} \cos^2 t d\sin t\\
&= -\int_0^{\pi} (1-\sin^2 t) d\sin t\\
&= -2\int_0^{\frac{\pi}{2}} (1-\sin^2 t) d\sin t\\
&= -2\int_0^1 (1-t^2) dt\\
&= -2(t-\frac{t^3}{3})|_0^3\\
&= -2(3-9)\\
&= 12
\end{align*}$$
*** c
$$\begin{align*}
\int_C xyz dz
&= \int_C xyz \cdot \frac{dz}{dt} dt\\
&= \int_0^{\pi} -\cos^2 t \sin t \cdot \sin t dt\\
&= -\int_0^{\pi} \cos^2 t \sin^2 t dt\\
&= -\frac{1}{4} \int_0^{\pi} \sin^2 2t dt\\
&= -\frac{1}{8} \int_0^{\pi} \sin^2 2t d2t\\
&= -\frac{1}{8} \int_0^{2\pi} \sin^2 t dt\\
&= -\frac{1}{8} \int_0^{2\pi} \frac{1-\cos 2t}{2} dt\\
&= -\frac{1}{16} \int_0^{2\pi} \frac{1-\cos 2t}{2} d2t\\
&= -\frac{1}{16} \int_0^{4\pi} \frac{1-\cos t}{2} dt\\
&= -\frac{1}{32} \int_0^{4\pi} 1-\cos t dt\\
&= -\frac{1}{32} (t-\sin t) |_0^{4\pi}\\
&= -\frac{1}{32} 4\pi\\
&= -\frac{\pi}{8}\\
\end{align*}$$
** 24
$$\begin{align*}
& C_1 &: r_1(t)=t\vec{i}\\
& C_2 &: r_2(t)=(1-t)\vec{i}+t\vec{j}\\
& C_3 &: r_3(t)=(1-t)\vec{j}
\end{align*}$$
where $0\leq t\leq 1$
$$\begin{align*}
\int_C (x-y)dx+(x+y)dy
&= \int_{C_1} (x-y)dx+(x+y)dy + \int_{C_2} (x-y)dx+(x+y)dy + \int_{C_3} (x-y)dx+(x+y)dy\\
&= \int_0^1 t dt + \int_0^1 2t dt + \int_0^1 t-1 dt\\
&= \int_0^1 4t-1 dt\\
&= 2\int_0^1 2t dt - 1\\
&= 2 t^2 |_0^1 - 1\\
&= 2 - 1\\
&= 1
\end{align*}$$
** 30
$$r(t)=a\cos t \vec{i} + a\sin t \vec{j}$$
$$r'(t)=-a\sin t \vec{i} + a\cos t \vec{j}$$
we use $Flux$ to denote flux
then
$$\begin{align*}
Flux_1
&= \int_C \vec{F}_1 dr\\
&= \int_0^{2\pi} (2x\vec{i}-3y\vec{j}) \cdot (-a\sin t \vec{i} + a\cos t \vec{j}) dt\\
&= \int_0^{2\pi} (2a\cos t \vec{i}-3a\sin t\vec{j}) \cdot (-a\sin t \vec{i} + a\cos t \vec{j}) dt\\
&= \int_0^{2\pi} -2.5a^2\sin 2t dt\\
&= \frac{5}{2} \int_0^{2\pi} a^2\sin 2t dt\\
&= \frac{5}{4} \int_0^{4\pi} a^2\sin t dt\\
&= \frac{5}{4}  a^2\cos t |_0^{4\pi}\\
&= 0
\end{align*}$$
$$\begin{align*}
Flax_2
&=  \int_C \vec{F}_1 dr\\
&=  \int_0^{2\pi} (2x\vec{i}+(x-y)\vec{j}) \cdot (-a\sin t \vec{i} + a\cos t \vec{j}) dt\\
&=  \int_0^{2\pi} (2a\cos t \vec{i}+a(\cos t-\sin t)\vec{j}) \cdot (-a\sin t \vec{i} + a\cos t \vec{j}) dt\\
&=  \int_0^{2\pi} -0.5a^2\sin 2t+a^2 \cos^2 t dt\\
&=  a^2 \int_0^{2\pi} -0.5\sin 2t+\cos^2 t dt\\
&=  a^2 \int_0^{2\pi} -0.5\sin 2t+\frac{1+\cos 2t}{2} dt\\
&=  a^2 \int_0^{2\pi} 0.5(-\sin 2t+\cos 2t + 1) dt\\
&=  a^2 \int_0^{4\pi} 0.5(-\sin t+\cos t + 1) dt\\
&= \frac{1}{2} a^2 \int_0^{4\pi} (-\sin t+\cos t + 1) dt\\
&= \frac{1}{2} a^2 (\cos t+\sin t+t)|_0^{4\pi}\\
&= \frac{1}{2} a^2 \left(4\pi + (\cos t+\sin t)|_0^{4\pi}\right)\\
&= 2\pi a^2
\end{align*}$$
** 36
$$\begin{align*}
& C_1 &: r_1(t)=(1-t)\vec{i}\\
& C_2 &: r_2(t)=-t\vec{i}\\
& C_3 &: r_3(t)=(1-t)\vec{i}+t\vec{j}\\
& C_4 &: r_4(t)=-t\vec{i}+(1-t)\vec{j}
\end{align*}$$
where $0\leq t\leq 1$
$$\begin{align*}
\int_C (x+y)dx-(x^2+y^2)dy
&= \int_{C_1} (x+y)dx-(x^2+y^2)dy + \int_{C_2} (x+y)dx-(x^2+y^2)dy + \int_{C_3} (x+y)dx-(x^2+y^2)dy + \int_{C_4} (x+y)dx-(x^2+y^2)dy\\
&= \int_{C_1} (x+y)dx-(x^2+y^2)dy + \int_{C_2} (x+y)dx-(x^2+y^2)dy + \int_{C_3} (x+y)dx-(x^2+y^2)dy + \int_{C_4} (x+y)dx-(x^2+y^2)dy\\
\end{align*}$$
** 42
** 48
** 54
** 60
