#+TITLE: Week 4.7 Math Homework
#+AUTHOR: 2024110144 陈有骏
#+LATEX_COMPILER: xelatex
#+LATEX_CLASS: article
#+LATEX_CLASS_OPTIONS: [a4paper,10pt]
#+LATEX_HEADER: \usepackage[margin=0.5in]{geometry}
#+LATEX_HEADER: \usepackage{xeCJK}
#+OPTIONS: \n:t toc:nil num:nil date:nil

#+begin_comment
4.7 done
thomas 15.6 1-20 mod 3
4.9 done
thomas 15.5 1-52 mod 5
4.11
thomas 15.7 1-66 mod 6
thomas 15.8 1-28 mod 7
#+end_comment

* 4.7
** 3
we can describe the region as $\int_0^2 \int_{4-y}^{\frac{y^2}{4}} dxdy$
which is
$$\begin{align*}
\int_0^2 \int_{4-y}^{\frac{y^2}{4}} dxdy &= \int_0^2 (\frac{y^2}{4} - (4-y)) dy\\
&= (\frac{y^3}{12} - 4y + \frac{y^2}{2})|_0^2\\
&= (\frac{8}{12} - 8 + \frac{4}{2})\\
&= \frac{2}{3} - 8 + 2\\
&= \frac{2}{3} - 6\\
&= -\frac{16}{3}
\end{align*}$$
to calculate the first moment of $x$
we have
$$\begin{align*}
\int_0^2 \int_{4-y}^{\frac{y^2}{4}} x dxdy &= \int_0^2 \frac{x^2}{2} |_{4-y}^{\frac{y^2}{4}} dy\\
&= \int_0^2 \frac{y^4}{32} - \frac{(4-y)^2}{2} dy\\
&= \frac{1}{2} \int_0^2 \frac{y^4}{16} - (4-y)^2 dy\\
&= \frac{1}{2} \int_0^2 \frac{y^4}{16} - (y^2-8y+16) dy\\
&= \frac{1}{2} \int_0^2 \frac{y^4}{16} - y^2 + 8y - 16 dy\\
&= \frac{1}{2} \left(- \frac{y^3}{3} + 4y^2 - 16y |_0^2\right)\\
&= \frac{1}{2} \left(- \frac{8}{3} + 16 - 32\right)\\
&= \frac{1}{2} \left(- \frac{8}{3} - 16\right)\\
&= -\frac{1}{2} \left(\frac{8}{3} + 16\right)\\
&= - \frac{4}{3} - 8\\
&= - \frac{28}{3}
\end{align*}$$
for the first moment of $y$
$$\begin{align*}
\int_0^2 \int_{4-y}^{\frac{y^2}{4}} y dxdy &= \int_0^2 y (\frac{y^2}{4} - (4-y)) dy\\
&= \int_0^2 y (\frac{y^2}{4} - 4 + y)) dy\\
&= \int_0^2 (\frac{y^3}{4} - 4y + y^2)) dy\\
&= (\frac{y^4}{16} - 2y^2 + \frac{y^3}{3})|_0^2\\
&= 1 - 8 + \frac{8}{3}\\
&= -7 + \frac{8}{3}\\
&= -\frac{13}{3}
\end{align*}$$
so the x-coordinate is $\frac{-\frac{28}{3}}{-\frac{16}{3}} = \frac{7}{4}$
the y-coordinate is $\frac{-\frac{13}{3}}{-\frac{16}{3}} = \frac{13}{16}$
so the desired coordinate is $(\frac{7}{4},\frac{13}{16})$

** 6
we can describe the region as $\int_0^{\pi} \int_0^{\sin x} dydx$
it is
$$\begin{align*}
\int_0^{\pi} \int_0^{\sin x} dydx &= \int_0^{\pi} \sin x dx\\
&= - \cos x |_0^{\pi}\\
&= \cos x |_{\pi}^0\\
&= 2
\end{align*}$$
the first moment of $x$ is
$$\begin{align*}
\int_0^{\pi} \int_0^{\sin x} x dydx
&= \int_0^{\pi} x\sin x dx\\
&= \int_0^{\pi} x\sin x dx\\
&= \sin x - x\cos x |_0^{\pi}\\
&= 0 - \pi (-1)\\
&= \pi
\end{align*}$$
the first moment of $y$ is
$$\begin{align*}
\int_0^{\pi} \int_0^{\sin x} y dydx
&= \int_0^{\pi} \frac{y^2}{2}|_0^{\sin x} dx\\
&= \int_0^{\pi} \frac{\sin ^2 x}{2} dx\\
&= \frac{1}{2} \int_0^{\pi} \sin ^2 x dx\\
&= \frac{1}{4} x-\frac{\sin 2x}{2}|_0^{\pi}\\
&= \frac{1}{4} \pi\\
&= \frac{\pi}{4}
\end{align*}$$
so the x-coordinate is $\frac{\pi}{2}$
the y-coordinate is $\frac{\pi}{8}$
the desired coordinate is $(\frac{\pi}{2},\frac{\pi}{8})$

** 9
we can describe the region as $\int_{-\infty}^0 \int_0^{e^x} dydx$
it is
$$\begin{align*}
\int_{-\infty}^0 \int_0^{e^x} dydx
&= \int_{-\infty}^0 e^x dx\\
&= \lim_{t\to -\infty} e^x |_t^0\\
&= \lim_{t\to -\infty} 1-e^t\\
&= 1-0\\
&= 1
\end{align*}$$

the first moment of $x$ is
$$\begin{align*}
\int_{-\infty}^0 \int_0^{e^x} x dydx
&= \int_{-\infty}^0 x e^x dx\\
&= (x-1) e^x|_{-\infty}^0\\
&= -1 + \infty \cdot e^{-\infty}\\
&= -1 + 0\\
&= -1
\end{align*}$$

the first moment of $y$ is
$$\begin{align*}
\int_{-\infty}^0 \int_0^{e^x} y dydx
&= \frac{1}{2} \int_{-\infty}^0 e^{2x} dx\\
&= \frac{1}{4} e^{2x}|_{-\infty}^0\\
&= \frac{1}{4} \cdot 1\\
&= \frac{1}{4}
\end{align*}$$

so the x-coordinate is $-1$
the y-coordinate is $\frac{1}{4}$
the desired coordinate is $(-1,\frac{1}{4})$

** 12
the coordinate of interpolate points are $(3,\pm \frac{\sqrt{3}}{2})$
so we have
$$\begin{align*}
\int_{-\frac{\sqrt{3}}{2}}^{\frac{\sqrt{3}}{2}} \int_{4y^2}^{\sqrt{12-4y^2}} \delta (x,y) dxdy
&= \int_{-\frac{\sqrt{3}}{2}}^{\frac{\sqrt{3}}{2}} \int_{4y^2}^{\sqrt{12-4y^2}} 5x dxdy\\
&= \int_{-\frac{\sqrt{3}}{2}}^{\frac{\sqrt{3}}{2}} \frac{5}{2} x^2 |_{4y^2}^{\sqrt{12-4y^2}} dy\\
&= 5 \int_{-\frac{\sqrt{3}}{2}}^{\frac{\sqrt{3}}{2}} 6-2y^2-8y^4 dy\\
&= 5 (6y-\frac{2}{3}y^3-\frac{8}{5}y^5) |_{-\frac{\sqrt{3}}{2}}^{\frac{\sqrt{3}}{2}}\\
&= 30y-\frac{10}{3}y^3-8y^5 |_{-\frac{\sqrt{3}}{2}}^{\frac{\sqrt{3}}{2}}\\
&= 30\sqrt{3}-\frac{5\sqrt{3}}{2}-\frac{9\sqrt{3}}{2}\\
&= 30\sqrt{3}-\frac{14\sqrt{3}}{2}\\
&= 23\sqrt{3}
\end{align*}$$

** 15
the total mass is
$$\begin{align*}
\int_0^6 \int_0^1 \delta (x,y) dydx
&= \int_0^6 \int_0^1 (x+y+1) dydx\\
&= \int_0^6 (x+\frac{3}{2}) dx\\
&= \int_0^6 x dx + 9\\
&= \frac{x^2}{2}_0^6 + 9\\
&= 18 + 9\\
&= 27
\end{align*}$$
the first moment of $x$ is
$$\begin{align*}
\int_0^6 \int_0^1 x \delta (x,y) dydx
&= \int_0^6 \int_0^1 x (x+y+1) dydx\\
&= \int_0^6 x \int_0^1 (x+y+1) dydx\\
&= \int_0^6 x (x+\frac{3}{2}) dx\\
&= \int_0^6 x^2 + \frac{3}{2} x dx\\
&= \frac{1}{3} x^3 + \frac{3}{4} x^2 |_0^6\\
&= 72 + 27\\
&= 99
\end{align*}$$
the first moment of $y$ is
$$\begin{align*}
\int_0^6 \int_0^1 y \delta (x,y) dydx
&= \int_0^6 \int_0^1 y (x+y+1) dydx\\
&= \int_0^6 \frac{x+1}{2} y^2 + \frac{1}{3} y^3 |_0^1 dx\\
&= \int_0^6 \frac{x+1}{2} + \frac{1}{3} dx\\
&= \frac{1}{2} \int_0^6 (x+1) dx + 2\\
&= \frac{1}{2} \int_0^6 x dx + 5\\
&= \frac{1}{4} x^2 |_0^6 + 5\\
&= 9 + 5\\
&= 14
\end{align*}$$
so the center of the mass is $(\frac{11}{3},\frac{14}{27})$
then we shall consider the moment of inertia about the y-axis
so we are rotating the thin rectangle by a stick of $x=\frac{11}{3}$
now, $0\leq x\leq 6$
we have
$$\begin{align*}
INERTIA_{y-axis} &= \int_0^6 \int_0^1 \delta (x,y) dy (x-\frac{11}{3})^2 dx\\
&= \int_0^6 (x+\frac{3}{2}) \cdot (x-\frac{11}{3})^2 dx\\
&= \int_0^6 (x+\frac{3}{2}) \cdot (x^2-\frac{22x}{3}+\frac{121}{9}) dx\\
&= \int_0^6 (x^3+\frac{3x^2}{2}-\frac{22x^2}{3}-11x+\frac{121x}{9}+\frac{121}{6}) dx\\
&= \int_0^6 (x^3-\frac{35x^2}{6}+\frac{22x}{9}+\frac{121}{6}) dx\\
&= (\frac{x^4}{4}-\frac{35x^3}{18}+\frac{11x^2}{9}+\frac{121x}{6})|_0^6\\
&= 324-420+44+121\\
&= 368-420+121\\
&= 489-420\\
&= 69
\end{align*}$$

** 18
the total mass
$$\begin{align*}
\int_0^{20} \int_{-1}^1 \delta (x,y) dydx
&= \int_0^{20} \int_{-1}^1 (1+\frac{x}{20}) dydx\\
&= \int_0^{20} (2+\frac{x}{10}) dx\\
&= (2x+\frac{x^2}{20})|_0^{20}\\
&= 40+20\\
&= 60
\end{align*}$$
the first moment of $x$
$$\begin{align*}
\int_0^{20} \int_{-1}^1 x\delta (x,y) dydx
&= \int_0^{20} \int_{-1}^1 (x+\frac{x^2}{20}) dydx\\
&= 2 \int_0^{20} (x+\frac{x^2}{20}) dx\\
&= 2 (\frac{x^2}{2}+\frac{x^3}{60})|_0^{20}\\
&= 2 (200+1200)\\
&= 2800
\end{align*}$$
the first moment of $y$
$$\begin{align*}
\int_0^{20} \int_{-1}^1 y\delta (x,y) dydx
&= \int_0^{20} \int_{-1}^1 (y+\frac{xy}{20}) dydx\\
&= \int_0^{20} (1+\frac{x}{20}) \int_{-1}^1 y dydx\\
&= \frac{1}{2} \int_0^{20} (1+\frac{x}{20}) y^2 |_{-1}^1 dx\\
&= \frac{1}{2} \int_0^{20} (1+\frac{x}{20}) 0 dx\\
&= 0
\end{align*}$$
the center of mass locates at $(\frac{140}{3},0)$
$$\begin{align*}
INERTIA_{y-axis} &= \int_0^{20} (x-\frac{140}{3})^2 \int_{-1}^1 \delta (x,y) dydx\\
&= 2 \int_0^{20} (x-\frac{140}{3})^2 (1+\frac{x}{20}) dx\\
&= 2 \frac{(x-\frac{140}{3})^3}{3} |_0^{20} + \frac{1}{10} \int_0^{20} x(x-\frac{140}{3})^2 dx\\
&= \frac{496000}{9} + \frac{1}{10} \int_0^{20} (x^3-\frac{280x^2}{3}+\frac{19600x}{9}) dx\\
&= \frac{496000}{9} + \frac{1}{10} (\frac{x^4}{4}-\frac{280x^3}{9}+\frac{9800x^2}{9})|_0^{20}\\
&= \frac{496000}{9} + \frac{1}{10} (40000-\frac{2240000}{9}+\frac{3920000}{9})\\
&= \frac{496000}{9} + \frac{1}{10} (40000+\frac{1680000}{9})\\
&= \frac{496000}{9} + \frac{1}{10} (40000+\frac{560000}{3})\\
&= \frac{496000}{9} + \frac{1}{10} \frac{680000}{3}\\
&= \frac{496000}{9} + \frac{68000}{3}\\
&= \frac{700000}{9}
\end{align*}$$

* 4.9
** 5
$$\int_{-2\sqrt{2}}^{2\sqrt{2}} \int_{-\sqrt{8-x^2}}^{\sqrt{8-x^2}} \left| \int_{x^2+y^2}^{8-x^2-y^2} dz \right| dydx$$
$$\int_{-2\sqrt{2}}^{2\sqrt{2}} \int_{-\sqrt{8-y^2}}^{\sqrt{8-y^2}} \left| \int_{x^2+y^2}^{8-x^2-y^2} dz \right| dxdy$$
$$\int_{-2\sqrt{2}}^{2\sqrt{2}} \left| \int_{x^2}^{8-x^2} \int_{z-x^2}^{8-x^2-z} dydz \right| dx$$
$$\int_{-2\sqrt{2}}^{2\sqrt{2}} \left| \int_{y^2}^{8-y^2} \int_{z-y^2}^{8-y^2-z} dxdz \right| dy$$
$$\int_0^8 \int_{-\sqrt{8-z}}^{\sqrt{8-z}} \int_{-\sqrt{8-x^2-z}}^{\sqrt{8-x^2-z}} dydxdz$$
$$\int_0^8 \int_{-\sqrt{8-z}}^{\sqrt{8-z}} \int_{-\sqrt{8-y^2-z}}^{\sqrt{8-y^2-z}} dxdydz$$
we would calculate the last one
$$\begin{align*}
\int_0^8 \int_{-\sqrt{8-z}}^{\sqrt{8-z}} \int_{-\sqrt{8-y^2-z}}^{\sqrt{8-y^2-z}} dxdydz
&= 2 \int_0^4 \pi z^2 dz\\
&= \frac{2\pi}{3} z^3 |_0^4\\
&= \frac{128\pi}{3}
\end{align*}$$
** 10
$$\begin{align*}
\int_0^1 \int_0^{3-3x} \int_0^{3-3x-y} dzdydx
&= \int_0^1 \int_0^{3-3x} 3-3x-y dydx\\
&= \int_0^1 (3-3x)y-\frac{y^2}{2} |_0^{3-3x} dx\\
&= \int_0^1 (3-3x)^2-\frac{(3-3x)^2}{2} dx\\
&= \int_0^1 \frac{(3-3x)^2}{2} dx\\
&= \frac{9}{2} \int_0^1 1-x dx\\
&= \frac{9}{4}
\end{align*}$$
** 15
$$\begin{align*}
\int_0^1 \int_0^{2-x} \int_0^{2-x-y} dzdydx
&= \int_0^1 \int_0^{2-x} 2-x-y dydx\\
&= \int_0^1 (2-x)y-\frac{y^2}{2}|_0^{2-x} dx\\
&= \int_0^1 \frac{(2-x)^2}{2} dx\\
&= \int_0^1 \frac{x^2}{2}-2x+2 dx\\
&= \frac{x^3}{6}-x^2+2x |_0^1\\
&= \frac{1}{6}-1+2\\
&= \frac{1}{6}+1\\
&= \frac{7}{6}
\end{align*}$$
** 20
$$\begin{align*}
\int_0^7 \int_0^2 \int_0^{\sqrt{4-q^2}} \frac{q}{r+1} dpdqdr
&= \int_0^7 \int_0^2 \frac{q\sqrt{4-q^2}}{r+1} dqdr\\
&= \int_0^7 \frac{1}{r+1} \int_0^2 q\sqrt{4-q^2} dqdr\\
&= \frac{1}{2} \int_0^7 \frac{1}{r+1} \int_0^2 \sqrt{4-q^2} dq^2dr\\
&= \frac{1}{2} \int_0^7 \frac{1}{r+1} \int_0^4 \sqrt{4-q} dqdr\\
&= -\frac{1}{2} \int_0^7 \frac{1}{r+1} \int_0^4 \sqrt{4-q} d(4-q)dr\\
&= \frac{1}{2} \int_0^7 \frac{1}{r+1} \int_0^4 \sqrt{q} dqdr\\
&= \frac{1}{3} \int_0^7 \frac{1}{r+1} q^{\frac{2}{3}} |_0^4 dr\\
&= \frac{1}{3} \int_0^7 \frac{1}{r+1} 4^{\frac{2}{3}} dr\\
&= \frac{1}{3} \int_0^7 \frac{1}{r+1} 4^{\frac{2}{3}} d(r+1)\\
&= \frac{1}{3} \int_1^8 \frac{1}{r} 4^{\frac{2}{3}} dr\\
&= \frac{4^{\frac{2}{3}}}{3} \int_1^8 \frac{1}{r} dr\\
&= \frac{4^{\frac{2}{3}}}{3} \ln r |_1^8\\
&= \frac{4^{\frac{2}{3}}}{3} \ln 8\\
&= 4^{\frac{2}{3}} \ln 2
\end{align*}$$
** 25
we can describe the region using
$$\int_0^2 \int_0^{2-z} \int_0^{4-y^2} dxdydz$$
so we can calculate it
$$\begin{align*}
\int_0^2 \int_0^{2-z} \int_0^{4-y^2} dxdydz
&= \int_0^2 \int_0^{2-z} 4-y^2 dydz\\
&= \int_0^2 4y-\frac{y^3}{3} |_0^{2-z} dz\\
&= \int_0^2 4(2-z)-\frac{(2-z)^3}{3} dz\\
&= \int_0^2 4z-\frac{z^3}{3} dz\\
&= 2z^2-\frac{z^4}{12} |_0^2\\
&= 8-\frac{4}{3}\\
&= \frac{20}{3}
\end{align*}$$
** 30
$$\begin{align*}
\int_0^2 \int_0^{4-x^2} \int_0^{4-x^2-y} dzdydx
&= \int_0^2 \int_0^{4-x^2} 4-x^2-y dydx\\
&= \int_0^2 4y- x^2 y - \frac{y^2}{2} |_0^{4-x^2} dx\\
&= \int_0^2 \frac{(4-x^2)^2}{2} dx\\
&= \int_0^2 \frac{x^4-8x^2+16}{2} dx\\
&= \int_0^2 \frac{x^4}{2}-4x^2+8 dx\\
&= \frac{x^5}{10}-\frac{4x^3}{3}+8x |_0^2\\
&= \frac{16}{5}-\frac{32}{3}+16\\
&= \frac{16}{5}-\frac{32}{3}+16\\
&= \frac{128}{15}
\end{align*}$$
#+begin_src scheme :exports both
  (+ 16/5 (- 32/3) 16)
#+end_src

#+RESULTS:
: 128/15

** 35
$$\begin{align*}
\int_{-1}^1 \int_{-\sqrt{4-4y^2}}^{\sqrt{4-4y^2}} \int_0^{x+2} dzdxdy
&= \int_{-1}^1 \int_{-\sqrt{4-4y^2}}^{\sqrt{4-4y^2}} x+2 dxdy\\
&= \int_{-1}^1 \frac{x^2}{2}+2x |_{-\sqrt{4-4y^2}}^{\sqrt{4-4y^2}} dy\\
&= \int_{-1}^1 4\sqrt{4-4y^2} dy\\
&= 8 \int_{-1}^1 \sqrt{1-y^2} dy\\
&= 8 \cdot \frac{1}{2} 1^2 \pi\\
&= 4\pi
\end{align*}$$
** 40
$$\begin{align*}
\int_0^2 \int_0^2 \int_0^2 xyz dxdydz
&= \int_0^2 \int_0^2 \frac{yzx^2}{2} |_0^2 dydz\\
&= \int_0^2 \int_0^2 2yz dydz\\
&= 2 \int_0^2 \int_0^2 yz dydz\\
&= 2 \int_0^2 \frac{zy^2}{2} |_0^2 dz\\
&= 2 \int_0^2 2z dz\\
&= 4 \int_0^2 z dz\\
&= 4 \frac{z^2}{2} |_0^2\\
&= 4 \cdot 2\\
&= 8
\end{align*}$$
** 45
the left part equals to
$$\begin{align*}
\int_0^1 \int_0^{4-a-x^2} \int_a^{4-x^2-y} dzdydx
&= \int_0^1 \int_0^{4-a-x^2} 4-x^2-y-a dydx\\
&= \int_0^1 (4-x^2-a)y - \frac{y^2}{2} |_0^{4-a-x^2} dx\\
&= \int_0^1 \frac{(4-a-x^2)^2}{2} dx\\
&= \frac{1}{2} \int_0^1 (4-a-x^2)^2 dx\\
&= \frac{1}{2} \int_0^1 (x^4-2(4-a)x^2+(4-a)^2) dx\\
&= \frac{1}{2} (\frac{x^5}{5}-\frac{2}{3} (4-a)x^3+(4-a)^2x)|_0^1\\
&= \frac{1}{2} (\frac{1}{5}-\frac{2}{3} (4-a) + (4-a)^2)\\
&= \frac{4}{15}
\end{align*}$$
which means
$$(4-a)^2-\frac{2}{3} (4-a)+\frac{1}{5}=\frac{8}{15}$$
$$(4-a)^2-\frac{2}{3} (4-a)+\frac{3}{15}=\frac{8}{15}$$
$$(4-a)^2-\frac{2}{3} (4-a)-\frac{1}{3}=0$$
so we have $4-a = \frac{\frac{2}{3}\pm\frac{4}{3}}{2} = \frac{1}{3}\pm\frac{2}{3}$
so $4-a=1,-\frac{1}{3}$
which means $a=3,4\frac{1}{3}$
since I think the question indicates that $4-a-x^2\geq 0$ even when negative integral might be valid as well
I shall only keep $a=3$

** 50
the triple integral is
$$\int_0^1 \int_{-\sqrt{z}}^{\sqrt{z}} \int_{-\sqrt{z-y^2}}^{\sqrt{z-y^2}} |xyz| dxdydz$$
#+begin_src python :python "python3" :results output :exports both
  from math import sqrt
  from scipy.integrate import tplquad

  result = tplquad (lambda x,y,z: abs(x*y*z), 0, 1, lambda z: -sqrt(z), lambda z: sqrt(z), lambda z,y: -sqrt(z-y**2), lambda z,y: sqrt(z-y**2))
  print(result)
#+end_src

#+RESULTS:
: (0.12499999999999997, 5.523359547510154e-15)
so the integral is $0.125$

* 4.11
** 15.7
*** 6
$$\begin{align*}
\int_0^{2\pi} \int_0^1 \int_{-\frac{1}{2}}^{\frac{1}{2}} (r^2\sin^2 \theta + z^2) dz rdr d\theta
&= \int_0^{2\pi} \int_0^1 (zr^2\sin^2 \theta + \frac{z^3}{3})|_{-\frac{1}{2}}^{\frac{1}{2}} rdr d\theta\\
&= 2 \int_0^{2\pi} \int_0^1 (zr^2\sin^2 \theta + \frac{z^3}{3})|_0^{\frac{1}{2}} rdr d\theta\\
&= \int_0^{2\pi} \int_0^1 (r^2\sin^2 \theta + \frac{1}{12}) rdr d\theta\\
&= \frac{1}{2} \int_0^{2\pi} \int_0^1 (r^2\sin^2 \theta + \frac{1}{12}) dr^2 d\theta\\
&= \frac{1}{2} \int_0^{2\pi} \int_0^1 (r\sin^2 \theta + \frac{1}{12}) dr d\theta\\
&= \frac{1}{4} \int_0^{2\pi} (r^2\sin^2 \theta + \frac{r}{6})|_0^1 d\theta\\
&= \frac{1}{4} \int_0^{2\pi} (\sin^2 \theta + \frac{1}{6}) d\theta\\
&= \frac{1}{4} \int_0^{2\pi} (\frac{1-\cos 2\theta}{2} + \frac{1}{6}) d\theta\\
&= \frac{1}{4} \int_0^{2\pi} (\frac{1}{2}-\frac{\cos 2\theta}{2} + \frac{1}{6}) d\theta\\
&= \frac{1}{4} (\frac{\theta}{2}-\frac{\sin 2\theta}{4} + \frac{\theta}{6}) |_0^{2\pi}\\
&= \frac{1}{4} (\frac{2\theta}{3}-\frac{\sin 2\theta}{4}) |_0^{2\pi}\\
&= \frac{1}{4} \frac{4\pi}{3}\\
&= \frac{\pi}{3}
\end{align*}$$

*** 12
so we have $z\geq r$ and $z\leq 2-r^2$
**** a
$$\int_0^{2\pi} \int_0^{\sqrt{2}} \int_r^{2-r^2} dzdrd\theta$$
**** b
$$\int_0^{2\pi} \int_0^2 \int_0^z drdzd\theta$$
**** c
$$\int_0^{\sqrt{2}} \int_r^{2-r^2} \int_0^{2\pi} d\theta dzdr$$

*** 18
we can use $r\sin\theta$ to represent $y$
so $z=3-r\sin\theta$
then the iterated integral can be
$$\int_0^{2\pi} \int_{\cos\theta}^{2\cos\theta} \int_0^{3-r\sin\theta} dzdrd\theta$$

*** 24
$$\begin{align*}
\int_0^{\frac{3\pi}{2}} \int_0^{\frac{\pi}{2}} \int_0^1 5\rho^3 \sin^3 \sigma d\rho d\sigma d\theta
&= 5 \int_0^{\frac{3\pi}{2}} \int_0^{\frac{\pi}{2}} \int_0^1 \rho^3 \sin^3 \sigma d\rho d\sigma d\theta\\
&= \frac{5}{4} \int_0^{\frac{3\pi}{2}} \int_0^{\frac{\pi}{2}} \rho^4 \sin^3 \sigma |_0^1 d\sigma d\theta\\
&= \frac{5}{4} \int_0^{\frac{3\pi}{2}} \int_0^{\frac{\pi}{2}} \sin^3 \sigma d\sigma d\theta\\
&= \frac{5}{4} \int_0^{\frac{\pi}{2}} \int_0^{\frac{3\pi}{2}} \sin^3 \sigma d\theta d\sigma\\
&= \frac{15\pi}{8} \int_0^{\frac{\pi}{2}} \sin^3 \sigma d\sigma\\
&= - \frac{15\pi}{8} \int_0^{\frac{\pi}{2}} \sin^2 \sigma d\cos\sigma\\
&= - \frac{15\pi}{8} \int_0^{\frac{\pi}{2}} 1 - \cos^2 \sigma d\cos\sigma\\
&= \frac{15\pi}{4} \int_0^1 1 - \sigma^2 d\sigma\\
&= \frac{15\pi}{4} \sigma - \frac{\sigma^2}{3} |_0^1\\
&= \frac{5\pi}{2}
$$\end{align*}

*** 30
$$\begin{align*}
\int_{\frac{\pi}{6}}^{\frac{\pi}{2}} \int_{-\frac{\pi}{2}}^{\frac{\pi}{2}} \int_{\csc \sigma}^2 5\rho^4 \sin^3 \sigma d\rho d\theta d\sigma
&= \int_{\frac{\pi}{6}}^{\frac{\pi}{2}} \int_{-\frac{\pi}{2}}^{\frac{\pi}{2}} \rho^5 \sin^3 \sigma |_{\csc \sigma}^2 d\theta d\sigma\\
&= \int_{\frac{\pi}{6}}^{\frac{\pi}{2}} \int_{-\frac{\pi}{2}}^{\frac{\pi}{2}} (32-\csc^5 \sigma) \sin^3 \sigma d\theta d\sigma\\
&= \int_{\frac{\pi}{6}}^{\frac{\pi}{2}} \pi (32-\csc^5 \sigma) \sin^3 \sigma d\sigma\\
&= \pi \int_{\frac{\pi}{6}}^{\frac{\pi}{2}} (32-\csc^5 \sigma) \sin^3 \sigma d\sigma\\
\end{align*}$$
no idea how to calculate the integral
*** 36
$$\begin{align*}
\int_0^{2\pi} \int_0^{\frac{\pi}{2}} \int_0^{1-\cos\sigma} d\rho d\sigma d\theta
&= \int_0^{2\pi} \int_0^{\frac{\pi}{2}} 1-\cos\sigma d\sigma d\theta\\
&= \int_0^{2\pi} \sigma-\sin\sigma |_0^{\frac{\pi}{2}} d\theta\\
&= \int_0^{2\pi} \frac{\pi}{2}-1 d\theta\\
&= \pi^2-2\pi
\end{align*}$$
*** 42
**** a
$$\int_0^{2\pi} \int_0^1 \int_0^1 r^2 dzdrd\theta$$
**** b
$$\int_0^{2\pi} \int_0^{\frac{\pi}{2}} \int_0^1 \rho^2 \cos^2 \sigma d\rho d\sigma d\theta$$
**** c
$$\begin{align*}
I_z &= \int_0^{2\pi} \int_0^1 \int_0^1 r^2 dzdrd\theta\\
&= \int_0^{2\pi} \int_0^1 r^2 drd\theta\\
&= \frac{1}{3} \int_0^{2\pi} r^3 |_0^1 d\theta\\
&= \frac{1}{3} \int_0^{2\pi} 1 d\theta\\
&= \frac{1}{3} \int_0^{2\pi} d\theta\\
&= \frac{2\pi}{3}
\end{align*}$$
*** 48
the upper cap is described by $z=3\sqrt{1-r^2}$
$$\begin{align*}
\int_0^{2\pi} \int_0^{|\cos \theta|} \int_0^{3\sqrt{1-r^2}} dzdrd\theta
&= \int_0^{2\pi} \int_0^{|\cos \theta|} 3\sqrt{1-r^2} drd\theta\\
&= 3\int_0^{2\pi} \int_0^{|\cos \theta|} \sqrt{1-r^2} drd\theta\\
&= 6\int_0^{\pi} \int_0^{\cos \theta} \sqrt{1-r^2} drd\theta\\
&= 6\int_0^{\pi} \int_0^{\arcsin \cos \theta} \cos u d\sin u d\theta\\
&= 6\int_0^{\pi} \int_0^{\arcsin \cos \theta} \cos^2 u du d\theta\\
&= 3\int_0^{\pi} \int_0^{\arcsin \cos \theta} (1+\cos 2u) du d\theta\\
&= 3\int_0^{\pi} \int_0^{2\arcsin \cos \theta} (1+\cos u) du d\theta\\
&= 3\int_0^{\pi} (u+\sin u)|_0^{2\arcsin \cos \theta} d\theta\\
&= 3\int_0^{\pi} (2\arcsin \cos \theta+\sin 2\arcsin \cos \theta) d\theta\\
&= 3\int_0^{\pi} (2\arcsin \cos \theta+\sin 2\arcsin \cos \theta) d\theta
\end{align*}$$
not able to proceed anymore
*** 54
we have $z=r^2$ as bottom
and $r=1$ as side
and $z=r^2+1$ as top
so
$$\begin{algin*}
\int_0^{2\pi} \int_0^1 \int_{r^2}^{r^2+1} dzdrd\theta
&= \int_0^{2\pi} \int_0^1 1 drd\theta\\
&= \int_0^{2\pi} \int_0^1 drd\theta\\
&= \int_0^{2\pi} 1 d\theta\\
&= \int_0^{2\pi} d\theta\\
&= 2\pi
\end{align*}$$
*** 60
we have $z=9-r^2,\,z\geq 0,\,r=1$
so
$$\begin{align*}
\int_0^{2\pi} \int_0^1 \int_0^{9-r^2} dzdrd\theta
&= \int_0^{2\pi} \int_0^1 9-r^2 drd\theta\\
&= \int_0^{2\pi} 9r-\frac{r^3}{3} |_0^1 d\theta\\
&= \int_0^{2\pi} 9-\frac{1}{3} d\theta\\
&= \frac{52\pi}{3}
\end{align*}$$
*** 66
$$\begin{align*}
\frac{\int_0^{2\pi} \int_0^{\frac{\pi}{2}} \int_0^1 d\rho d\sigma d\theta}{\int_0^{2\pi} \int_0^{\frac{\pi}{2}} \int_0^1 \rho \cos \sigma d\rho d\sigma d\theta}
&= 2 \frac{\int_0^{2\pi} \int_0^{\frac{\pi}{2}} d\sigma d\theta}{\int_0^{2\pi} \int_0^{\frac{\pi}{2}} \cos \sigma d\sigma d\theta}\\
&= 2 \frac{\int_0^{2\pi} \frac{\pi}{2} d\theta}{\int_0^{2\pi} 1 d\theta}\\
&= \pi \frac{\int_0^{2\pi} d\theta}{\int_0^{2\pi} d\theta}\\
&= \pi \cdot 1\\
&= \pi
\end{align*}$$
** 15.8
*** 7
$$u=3x+2y,\,v=x+4y$$
the Jacobian determinant is
$$\left|\begin{matrix} 3 & 2 \\ 1 & 4 \end{matrix}\right| = 12 - 2 = 10$$
using $u,v$ to represent $x,y$, we have
$$\left{\begin{align*}
& x &= \frac{2u-v}{5}\\
& y &= \frac{3v-u}{10}
\end{align*}\right .$$
so the integral becomes $\int\int_{R_{u,v}} (3x^2+14xy+8y^2) \cdot 10 dudv$
$$3x^2+14xy+8y^2 = 3(\frac{2u-v}{5})^2 + 14 \frac{2u-v}{5} \frac{3v-u}{10} + 8(\frac{3v-u}{10})^2$$
also the lines should be transfromed
not able to proceed because it seems too difficult for me
*** 14
the Jacobian determinant is
$$\left|\begin{matrix} 1 & \frac{1}{2} \\ 0 & 1\end{matrix}\right| = 1$$
then the integral becomes
$$\int_0^2 \int_0^2 2v^3 ue^{4u^2} dudv$$
so we can evaluate this as
$$\begin{align*}
\int\int_{G:\text{a region bond by line u=0,2 and line v=0,2}} 2v^3 ue^{4u^2} dudv
&= \int_0^2 \int_0^2 2v^3 ue^{4u^2} dudv\\
&= \int_0^2 2v^3 \int_0^2 ue^{4u^2} dudv\\
&= \frac{1}{8} \int_0^2 2v^3 e^{4u^2}|_0^2 dv\\
&= \frac{1}{8} \int_0^2 2v^3 (e^{16}-1) dv\\
&= \frac{e^{16}-1}{4} \int_0^2 v^3 dv\\
&= \frac{e^{16}-1}{16} v^4 |_0^2\\
&= e^{16}-1
\end{align*}$$
*** 21
**** a
$$\left|\begin{matrix} \cos v & -u\sin v \\ \sin v & u\cos v\end{matrix}\right| = u$$
**** b
$$\left|\begin{matrix} \sin v & u\cos v \\ \cos v & -u\sin v\end{matrix}\right| = -u$$
*** 28
we have $x=\sqrt{\frac{u}{v}},y=\sqrt{uv}$
so the lines are $v=2,v=\frac{1}{2},u=2,u=\frac{1}{2}$
and $y^2=uv$
we have
$$\begin{align*}
\int\int_R y^2 dA
&= \int_{\frac{1}{2}}^2 \int_{\frac{1}{2}}^2 uv dudv\\
&= \frac{1}{2} \int_{\frac{1}{2}}^2 u^2 v |_{\frac{1}{2}}^2 dv\\
&= \frac{1}{2} \int_{\frac{1}{2}}^2 (4-\frac{1}{4}) v dv\\
&= (2-\frac{1}{8}) \int_{\frac{1}{2}}^2 v dv\\
&= (1-\frac{1}{16}) v^2 |_{\frac{1}{2}}^2\\
&= (1-\frac{1}{16}) (4-\frac{1}{4})\\
&= \frac{15}{16}\cdot\frac{15}{4})\\
&= \frac{225}{64}
\end{align*}$$
