#+TITLE: 11.27math
#+AUTHOR: 2024110144

* Question 1
Suppose $f(x) = x^4 - 5x^3 + x^2 - 3x + 4$
- $f'(x) = 4x^3 - 15x^2 + 2x - 3$
- $f"(x) = 12x^2 - 30x + 2$
- $f^{(3)}(x) = 24x - 30$
- $f^{(4)} = 24$
Thus the answer is $-56 + 21(x-4) + 37(x-4)^2 + 11(x-4)^3 + 24(x-4)^4$

* Question 3
- $y' = \sec^2 x$
- $y" = 2\sin x \sec^3 x$
Thus the answer is $y = x$

* Question 5
- $y' = -{1 \over x^2}$
- $y" = {2 \over x^3}$
- $y^{(3)} = -{6 \over x^4}$
- $y^{(n)} = (-1)^n \frac{n!}{x^{n+1}}$
Applying Taylor Formula, we get $y = \sum_{i=0}^n \frac{(-1)^n}{x^{n+1}}(x+1)^i$

* Question 7
My answer is $1 + {1 \over 2} x^2 + ... + {2 \over (2n)!} x^{2n}$

* Question 13
** Question (1)
- $(\sin x)' = \cos x$
- $(\sin x)" = -\sin x$
- $(\sin x)^{(3)} = -\cos x$
- $(\sin x)^{(4)} = \sin x$
Thus we can use the approximation at $x_0$ as \( \sin x = \sin x_0 + \cos x_0 (x - x_0) - \frac{\sin x_0}{2} (x - x_0)^{2} - \frac{\cos x_0}{6} (x - x_0)^{(3)} + ... \)

Take $x_0 = 0$ into the equation we get \( \sin x = x + ... \)

Thus the answer is approximately $0.31459265358979$

The deviation is about $10^{-4}$
** Question (2)
Suppose $f(x) = \sqrt{x}$

Then we have
- $f'(x) = \frac{1}{2\sqrt{x}}$
- $f"(x) = - \frac{1}{4(\sqrt{x})^3}$
- $f^{(3)} (x) = \frac{3}{8 x^{\frac{5}{2}}}$
Thus we have the expansion with $x_0 = 9$ as $f(x) = 3 + \frac{1}{6} (x - 9) - \frac{1}{216} (x - 9)^2 + \frac{1}{3888} (x - 9)^3$

So our approximation would be $3 + \frac{1}{6} - \frac{1}{216} + \frac{1}{3888}$

The deviation is about $10^{-3}$
** Question (3)
Suppose $f(x) = \ln (1+x)$

Then we have
- $f'(x) = \frac{1}{1+x}$
- $f"(x) = -\frac{1}{(1+x)^2}$
- $f^{(3)} = \frac{2}{(1+X)^3}$
Thus we have the expansion with $x_0 = 0$ as $f(x) = x - \frac{1}{2} x^2 + \frac{1}{3} x^3$

So the answer is $0.2 - 0.02 + \frac{0.008}{3}$

Which is about $0.1826666666666667$

The deviation is about $10^{-4}$
** Question (4)
Suppose $f(x) = \root 3 \of {x}$

Then we have
- $f'(x) = \frac{1}{3} x^{-\frac{2}{3}}$
- $f"(x) = -\frac{2}{9} x^{-\frac{5}{3}}$
- $f^{(3)}(x) = \frac{10}{27} x^{-\frac{8}{3}}$

Thus we have the expansion with $x_0 = 27$ as $f(x) = 3 + \frac{1}{27} (x-27) - \frac{1}{3^7} (x-27)^2 + \frac{5}{3^{12}} (x-27)^3$

So the answer is $3 + \frac{1}{9} - \frac{1}{3^5} + \frac{5}{3^9}$

Which is about $3.107249911090789$

The deviation is about $10^{-4}$
* Question 17
** Question (3)
The limit equals to $\lim_{x \to 0} \frac{1 - \frac{x^4}{2} + o(x^4) - x^2 + \frac{x^4}{2} - x^2 o(x^2) - 1}{x^2} = \lim_{x \to 0} \frac{o(x^4)}{x^2} = 0$
** Question (6)
The limit equals to$\lim_{x \to 0} \frac{1 - e^{\sin x \ln \cos x}}{x^3} = \lim_{x \to 0} - \frac{\sin x \ln \cos x}{x^3}$

$= \lim_{x \to 0} \frac{1 - e^{\frac{x^3}{2} - \frac{x^5}{8} - \frac{x^5}{12} + \frac{x^7}{40}}}{x^3} = \frac{1}{2}$
** Question (9)
The limit equals to

$\lim_{x \to 0} \frac{x + \frac{x^3}{3} + o(x^2) - \frac{\left(x + \frac{x^3}{3} + o(x^n)\right)^3}{6} + o \left(x + \frac{x^3}{3} + o(x^n)\right)^n - \left(x - \frac{x^3}{6} + o(x^n)\right) - \frac{\left(x + \frac{x^3}{6} + o(x^n)\right)^3}{3} - o \left(x - \frac{x^3}{6} + o(x^n)\right)^n}{x^7}$

$= -\frac{1}{30}$
** Question (12)
The limit equals to

$\lim_{x \to 1} \frac{\alpha^2 \left(\beta x + \beta x^2 + o (x-1)^n\right) - \beta^2 \left(\alpha x + \alpha x^2 + o (x-1)^n\right)}{\left(\alpha x + \alpha x^2 + o (x-1)^n\right)\left(\beta x + \beta x^2 + o (x-1)^n\right)}$

$= \frac{\alpha - \beta}{2}$
