#+TITLE: Week 9.15 Math Homework
#+AUTHOR: 2024110144 陈有骏
#+LATEX_COMPILER: xelatex
#+LATEX_CLASS: article
#+LATEX_CLASS_OPTIONS: [a4paper,10pt]
#+LATEX_HEADER: \usepackage[margin=0.5in]{geometry}
#+LATEX_HEADER: \usepackage{xeCJK}
#+LATEX_HEADER: \usepackage{fontspec}
#+LATEX_HEADER: \setCJKmainfont{WenQuanYi Zen Hei}
#+OPTIONS: \n:t toc:nil num:nil date:nil

#+begin_comment
9.15 2.4 Problems 1-27 mod 5 P71
9.17 2.5 Problems 1-27 mod 5
#+end_comment

* 9.15
** 5
#+begin_comment
Theorem 2.4.2
Existence and Uniqueness Theorem for First-Order Nonlinear Equations
#+end_comment
$y'=(1-t^2-y^2)^{\frac{1}{2}}$
when $0<t<\frac{\sqrt{2}}{2}, 0<y<\frac{\sqrt{2}}{2}$
there is only one solution

** 10
$y'=2ty^2$
obsolutely $y=0$ for $t$ is a solution
then when $y\neq 0$, we have $y^{-2}y'=2t$
so $(-y^{-1})'=2t$
so $-y^{-1}=t^2+C$
which means $\frac{1}{y}+t^2+C=0$
apply $y(0)=y_0$, we know $C=-\frac{1}{y_0}$
which gives the second answer, $\frac{1}{y}+t^2-\frac{1}{y_0}=0$
so when $y_0=0, y=0$ for all $t$
when $y_0\neq 0, \frac{1}{y}+t^2-\frac{1}{y_0}=0$ for all $t$

** 15
the direction field is
[[file:images/9.15-15/output.png]]
one solution is of course $y=0$
when $y\neq 0$, suppose $y(0)=y_0$
we know $y'=-y(3-ty)$
then $y'+3y=ty^2$, a Bernoulli equation
so we have $y^{-2}y'+3y^{-1}=t$
then $(-1)(y^-1)'+3y^{-1}=t$
we wish there is a $u(t)$ to have $u'(t)=-3u(t)$
seemingly $u(t)=e^{-3t}$ makes sense
so $e^{-3t}(y^{-1})'+(e^{-3t})'y^{-1}=-te^{-3t}$
then the left part can be rewritten as $(e^{-3t}y^{-1})'$
so $$\begin{align*}
e^{-3t}y^{-1}  &= \int -te^{-3t} dt\\
&= \int -t \cdot (-\frac{1}{3}) de^{-3t}\\
&= \frac{1}{3} \int t \cdot de^{-3t}\\
&= \frac{1}{3} \left(te^{-3t}- \int e^{-3t} dt\right)\\
&= \frac{1}{3} \left(te^{-3t}- [(-3) e^{-3t} + C]\right)\\
&= \frac{1}{3} \left(te^{-3t} + 3 e^{-3t} - C\right)\\
&= \frac{1}{3} (t+3)e^{-3t} + \frac{1}{3}C\\
&= \frac{1}{3} (t+3)e^{-3t} + C
\end{align*}$$
so $\frac{1}{y}=1 + \frac{t}{3} + Ce^{3t}$
when $y(0)=y_0$, we know $\frac{1}{y_0}=1 + C$
giving $C= \frac{1}{y_0}-1$
$$\frac{1}{y}=1 + \frac{t}{3} + (\frac{1}{y_0}-1)e^{3t}$$
#+begin_src gnuplot :file 9.15-2.4-15.png :exports both
  set xrange [0:0.5]
  set yrange [0:40]
  set xlabel "x"
  set ylabel "y"
  set title "9.15-2.4-15"

  f(x, y_0)=1.0/(1+x/3+(1.0/y_0-1)*exp(3*x))
  f_1(x)=f(x, 1)
  f_2(x)=f(x, 2)
  f_3(x)=f(x, 3)
  f_5(x)=f(x, 5)

  plot f_1(x) title "y(0)=1", f_2(x) title "y(0)=2", f_3(x) title "y(0)=3",f_5(x) title "y(0)=5"
#+end_src

#+RESULTS:
[[file:9.15-2.4-15.png]]

when $y_0=1$, the solution is a line down
when $y_0>1$, the solution is larger and larger as $y_0$ gets larger
when $y_0<1$, of course it is smaller, even negative

** 20
given $\phi '(t) + p(t)\phi (t)=0$
then $$\begin{align*}
(c\phi (t))' + p(t) (c\phi (t)) &= c\phi '(t) + cp(t)\phi (t)\\
&= c(\phi '(t) + p(t)\phi (t))
\end{align*}$$
when $c=0$, of course
when $c\neq 0$, since $\phi '(t) + p(t)\phi (t)=0$, still zero

** 25
$y^{-3}y'-\epsilon y^{-2}=-\delta$
since $(y^{-2})' = -2y^{-3}y'$
so $(y^{-2})'+2\epsilon y^{-2}=2\delta$
then $$\begin{align*}
y^{-2}e^{2\epsilon t}
&= \int 2\delta e^{2\epsilon t} dt\\
&= 2\delta \int e^{2\epsilon t} dt\\
&= \frac{\delta}{\epsilon} e^{2\epsilon t} + C
\end{align*}$$
so $y^{-2}=\frac{\delta}{\epsilon} + Ce^{-2\epsilon t}$

* 9.17
** 5
*** a
we let $y'=0$, then only $y=1$ suits
which means $y=1$ is the only critical point
and when $y=1, y'=0$, we have $y=1$ for any $t$
meaning $\phi (t)=1$
*** b
don't understand what it means by "sketch f(y) versus y"
what is "f(y)"?
when $y\neq 1$, $y'=k(1-y)^2>0$, meaning $y(t)$ is increasing
*** c
$$\frac{dy}{(1-y)^2}=kdt, k>0$$
let $m=1-y
$$-\int \frac{dm}{m^2}=kt+C$$
$$\frac{1}{m}=kt+C$$
$$\frac{1}{1-y}=kt+C$$
when $y\neq 1$, $y=1-\frac{1}{kt+C}$
apply $y_0$ we have $C=\frac{1}{1-y_0}$
so $y=1-\frac{1}{kt+\frac{1}{1-y_0}}$
when $y_0>1$, $y>1$, $y'>0$
when $y_0<1$, $y<1$, $y'>0$, $y\to 1$
so it is semistable, the conclusions in (b) are correct

** 10
#+begin_comment
Complete the derivation of the explicit formula
for the solution (11) of the logistic model
by solving equation (10) for y.

equation (10):
$\frac{y}{1-\frac{y}{k}} = Ce^{rt}$

solution (11):
$y = \frac{y_0 K}{y_0 + (K - y_0) e^{-rt}$

the logistic model:
to satisfy the initial condition,
we must choose $C=\frac{y_0}{1-\frac{y_0}{k}}$
#+end_comment
take $C$ in, we have $\frac{y}{1-\frac{y}{k}} = \frac{y_0}{1-\frac{y_0}{k}}e^{rt}$
when $y=0$, $y_0=0$
when $y\neq 0$, $\frac{1}{\frac{1}{y} - \frac{1}{k}}=\frac{y_0}{1-\frac{y_0}{k}}e^{rt}$
so $\frac{1}{y} - \frac{1}{k}=\frac{1-\frac{y_0}{k}}{y_0e^{rt}}$
then $\begin{align*}
\frac{1}{y} &= \frac{k-y_0}{ky_0e^{rt}}+\frac{1}{k}\\
&= \frac{k-y_0+y_0e^{rt}}{ky_0e^{rt}}
\end{align*}$
so $\begin{align*}
y &= \frac{ky_0e^{rt}}{k-y_0+y_0e^{rt}}\\
&= \frac{ky_0}{(k-y_0)e^{-rt}+y_0}\\
&= \frac{ky_0}{y_0 + (k-y_0)e^{-rt}}
\end{align*}$

** 15
$dy\cdot \frac{1}{y(K-y)} = \frac{r}{K}dt$
we wish $\frac{1}{y(K-y)}=\frac{A}{y}+\frac{B}{K-y}$
so $1=KA-yA+yB$
which requires $\begin{align*}
A &= \frac{1}{K}\\
B &= \frac{1}{K}
\end{align*}$
so $dy\cdot (\frac{1}{y}+\frac{1}{K-y}) = rdt$
integrate both sides for $t$
we have $\ln |y| - \ln |K-y| = rt +C$
which means $\frac{|y|}{|K-y|}=e^{rt+C}$
so $|\frac{1}{\frac{K}{y}-1}|=e^{rt}+C$
then $|y|=\frac{K}{1+\frac{1}{e^{rt}+C}}$
apply $t=0, y=y_0$
we have $|y_0|=\frac{K}{1+\frac{1}{1+C}}$
so $C=\frac{1}{frac{K}{|y_0|}-1}-1$
then $|y|=\frac{K}{1+\frac{1}{e^{rt}+\frac{1}{frac{K}{|y_0|}-1}-1}}$
since the equation is used to describe population
we can suppose $y\geq 0$
so $y=\frac{K}{1+\frac{1}{e^{rt}+\frac{1}{frac{K}{y_0}-1}-1}}$
*** a
$y=\frac{K}{1+\frac{1}{e^{rt}-\frac{1}{2}}}$
we want $\tau$ that
$$\begin{align*}
\frac{2K}{3} &= \frac{K}{1+\frac{1}{e^{r\tau}-\frac{1}{2}}}\\
\frac{2}{3} &= \frac{1}{1+\frac{1}{e^{r\tau}-\frac{1}{2}}}\\
2 (e^{r\tau}-\frac{1}{2}) &= 3\\
e^{r\tau}-\frac{1}{2} &= \frac{3}{2}\\
e^{r\tau} &= 2\\
r\tau &= \ln 2\\
\tau &= \frac{\ln 2}{r}
\end{align*}$$
when $r=0.025$,  $\tau=40\ln 2$
which is about $27.725887222397812$ by calculator
*** b
$y=\frac{K}{1+\frac{1}{e^{rt}+\frac{1}{\frac{1}{\alpha}-1}-1}}$
apply the condition, we have
$$\begin{align*}
\beta &= \frac{1}{1+\frac{1}{e^{rT}+\frac{1}{\frac{1}{\alpha}-1}-1}}\\
\frac{1}{\beta} &= 1+\frac{1}{e^{rT}+\frac{1}{\frac{1}{\alpha}-1}-1}\\
\frac{1}{\beta}-1 &= \frac{1}{e^{rT}+\frac{1}{\frac{1}{\alpha}-1}-1}\\
\frac{1}{\frac{1}{\beta}-1} &= e^{rT}+\frac{1}{\frac{1}{\alpha}-1}-1\\
\frac{1}{\frac{1}{\alpha}-1}-\frac{1}{\frac{1}{\beta}-1} &= 1-e^{rT}\\
\frac{\alpha}{1-\alpha}-\frac{\beta}{1-\beta} &= 1-e^{rT}\\
\frac{\alpha-\beta}{(1-\alpha)(1-\beta)} &= 1-e^{rT}\\
e^{rT} &= \frac{1-2\alpha+\alpha\beta}{(1-\alpha)(1-\beta)}\\
rT &= \ln |\frac{1-2\alpha+\alpha\beta}{(1-\alpha)(1-\beta)}|\\
T &= \frac{1}{r} \ln |\frac{1-2\alpha+\alpha\beta}{(1-\alpha)(1-\beta)}|\\
\end{align*}$$
when $\alpha\to 0$, $T\to \frac{1}{r} \ln |1-\beta|$
further more, when $\beta\to 1$, $T\to \infty$
applying the values
we get $T=40\ln |\frac{0.89}{0.09}|$
which evaluates to $T=40\ln 89 - 80\ln 3$
which is approximately $91.65647169583681$ by calculator

** 20
$$\begin{align*}
y' &= ry-\frac{r}{K}y^2-h\\
y^{-2}y'-ry^{-1} &= -\frac{r}{K}-hy^{-2}\\
(y^{-1})'+ry^{-1} &= \frac{r}{K}+hy^{-2}\\
\frac{d(y^{-1}e^{rt})}{dt} &= e^{rt}\frac{r}{K}+hy^{-1}\cdot y^{-1}e^{rt}
\end{align*}
suppose $m=y^{-1}e^{rt}$, $C_1=e^r\frac{r}{K}$, $C_2=he^{-r}$
$$\frac{dm}{dt} = C_1 e^t + C_2 m^2 e^{-t}$$
this is not linear, not knowing how to solve this
*** a
$$\begin{align*}
(1-\frac{y}{K})y &= h\
(K-y)y &= Kh\\
y^2-Ky+Kh &= 0
\end{align*}$$
since $\delta=K^2-4Kh>0$
we know there are two equilibrium points
$$\begin{align*}
y_1 &= \frac{K-\sqrt{K^2-4Kh}}{2}\\
y_2 &= \frac{K+\sqrt{K^2-4Kh}}{2}
\end{align*}$$
*** b
when $y<y_1$, $y'<0$
when $y_2>y>y_1$, $y'>0$
when $y_2<y$, $y'<0$
so $y_1$ is unstable, $y_2$ is asymtotically stable
*** c
no idea what $f(y)$ means!
when $y<y_1$, $y \to -\infty$
when $y_2>y>y_1, t\to\infty$,
since there is no other equilibruim point between, it would goto $y_2$,
the next equilibruim point
*** d
$\delta < 0$, there is no equilibruim point at all, and $y'<0$
so $y$ would go all the way down, but since in reallity, $y\geq 0$
so it would at some time becomes $0$
*** e
of course because $\delta=0$ and $y_0=\frac{K}{2}$
when $y\neq y_0$, $y'<0$, so it is semistable

** 25
$\frac{dy}{dt}=ay-y^3=y(a-y^2)$
when $a \leq 0$, there is only one critical point, $y=0$
when $a > 0$, there are two, $y=0$ or $y=\sqrt{a}$

