#+TITLE: Week 9.8 Math Homework
#+AUTHOR: 2024110144 陈有骏
#+LATEX_COMPILER: xelatex
#+LATEX_CLASS: article
#+LATEX_CLASS_OPTIONS: [a4paper,10pt]
#+LATEX_HEADER: \usepackage[margin=0.5in]{geometry}
#+LATEX_HEADER: \usepackage{xeCJK}
#+LATEX_HEADER: \usepackage{fontspec}
#+LATEX_HEADER: \setCJKmainfont{WenQuanYi Zen Hei}
#+OPTIONS: \n:t toc:nil num:nil date:nil

#+begin_comment
9.8 1.1 Problems  2.1 1-30 mod 5
9.10 1.2 Problems 2.2 &2.3 1-24 mod6
#+end_comment

* 9.8
** 5
$y'-2y=3e^t$
*** the direction field
[[file:images/9.8-5/output.png]]
*** how solutions behave for large $t$
solutions become positive infinity for all $y$ when $t$ is large
*** the general solution and how solutions behave for large $t$
$P(t)=-2, Q(t)=3e^t$
for $y'+P(x)y=Q(x)$
we know $y=Ce^{-\int P(x)dx}$
then $y'=C'e^{-\int P(x)dx}-CP(x)e^{-\int P(x)dx}$
so $Q(x)=C'e^{-\int P(x)dx}$
thus $C'=Q(x)e^{\int P(x)dx}$
$C=\int Q(x)e^{\int P(x)dx}$
so the integrating factor is $e^{\int P(x)dx}=e^{-2t}$
then $e^{-2t}y'-2e^{-2t}y=3e^{-t}$
so $\frac{d(e^{-2t}y)}{dt}=3e^{-t}$
then $\int \frac{d(e^{-2t}y)}{dt} dt = \int 3e^{-t} dt$
we get $e^{-2t}y=-3e^{-t}+C$
so $y=-3e^t+Ce^{2t}$
when t is really large, it depends on $C$
if $C$ is zero or negative, it goes negative infinity
if $C$ is positive, it goes positive infinity

** 10
$y'+2y=te^{-2t}, y(1)=0$
$P(t)=2, Q(t)=te^{-2t}$
then factor is $e^{\int P(t)dt}= e^{2t}$
we have $e^{2t}y'+2e^{2t}y=t$
then $\frac{d(e^{2t}y)}{dt}=t$
$e^{2t}y=\int t dt$
$e^{2t}y=\frac{1}{2} t^2 + C$
$y=\frac{1}{2} t^2e^{-2t}+Ce^{-2t}$
apply $y(1)=0$, we have $\frac{1}{2}e^{-2}+Ce^{-2}=0$
so $C=-\frac{1}{2}$
$y=\frac{1}{2} t^2e^{-2t}-\frac{1}{2}e^{-2t}$

** 15
$ty'+(t+1)y=2te^{-t},y(1)=a,t>0$
the direction field is
[[file:images/9.8-15/output.png]]
when $t\to 0$ it behaves like nothing?
does not depend on initial value $a$ of course
I don't know where $a_0$ should be from my picture
$P(t)=1+\frac{1}{t}, Q(t)=2e^{-t}$
integrating factor is $e^{\int P(t) dt}$
which is $e^{t+\ln t}$
so $e^{t+\ln t}y' + (1+\frac{1}{t})e^{t+\ln t}y = 2t$
$te^ty = t^2+C$
$y=te^{-t}+\frac{C}{te^t}$
now $\frac{C+1}{e}=a$, so $C=ae-1$
$y=te^{-t}+\frac{ae-1}{te^t}$
when $t\to \infty$, y approaches $0$ with the symbol of $ae-1$
so $a_0=\frac{1}{e}$
when $a$ is smaller than $a_0$ it approaches $0^-$
else, $0^+$.

** 20
$y'-y=1+3\sin t, y(0)=y_0$
$P(t)=-1, Q(t)=1+3\sin t$
factor is $e^{-t}$
so $e^{-t}y=\int (1+3\sin t) e^{-t}$
don't know how to integrate the right part..

** 25
#+begin_comment
All solutions are symptotic to the line y=3-t as t \to \infty
Construct a first-order differencial equation that suits this and then solve it to prove.
#+end_comment
$y'+P(t)y=Q(t)$
let $P(t)=1, Q(t)=4-t$
we have factor as $e^t$
then $e^ty=\int (4-t)e^t dt$
$e^ty=4e^t-\int te^t dt$
since $\int \frac{t}{e^t} dt = \int t de^t = te^t-\int e^{-t} dt = -(t+1)e^{-t} + C$
we have $y=-4-(t+1)+Ce^t=t-3+Ce^{-t}$
which is obviously symptotic to $y=t-3$

** 30
$y'+\frac{1}{t}y=\cos (2t), t>0$
$y=\frac{1}{t} (\int t\cos(2t) dt)$
$$\begin{align*}
\int t\cos(2t) dt &= \int t d \frac{1}{2}\sin (2t)\\
&= \frac{1}{2} \int t d \sin (2t)\\
&= \frac{1}{2} \left(t\sin (2t) - \int \sin (2t) dt\right)\\
&= \frac{1}{2} \left(t\sin (2t) + 2\cos (2t)\right) + C\\
&= \frac{1}{2} t\sin (2t) + \cos (2t) + C
\end{align*}$$
$y=\frac{1}{2} \sin (2t) + \frac{1}{t}\cos (2t) +C$

* 9.10
** 2.2
*** 6
$\frac{dy}{dx}=\frac{x^2}{1+y^2}$
$(1+y^2)dy=x^2dx$
$3y+y^3=x^3+C$
*** 12
$\frac{1}{r^2}dr=\frac{1}{\theta}d\theta$
$-\frac{1}{r}=\ln\theta + C$
$C=-\frac{1}{2}$
$\frac{1}{r}+\ln\theta-\frac{1}{2}=0$
#+begin_src gnuplot :file 9.10-2.2-12.png :exports both
  set xrange [0:2 * pi]
  set yrange [-10:10]
  set xlabel "theta"
  set ylabel "r"
  set title "9.10-2.2-12"

  f(x)=1.0 / (0.5 - log (x))

  plot f(x) notitle
#+end_src

#+RESULTS:
[[file:9.10-2.2-12.png]]

from the picture, the solution is defined in $(0, 2.4)$ and $(2.7, +\infty)$

*** 18
$(3y^2-4)dy=3x^2dx$
$y^3-4y=x^3+C$
$0=1+C$ gives $C=-1$
so $y^3-4y-x^3+1=0$
it is defined on $(-\infty,-\frac{2\sqrt{3}}{3})\cup (-\frac{2\sqrt{3}}{3},\frac{2\sqrt{3}}{3})\cup (\frac{2\sqrt{3}}{3},+\infty)$
*** 24
$\frac{1}{a+bQ}dQ=rdt$
$\ln |a+bQ| = brt +C$
$C= \ln |a+bQ_0|$
$\ln |a+bQ| = brt +\ln |a+bQ_0|$
$|a+bQ|=|a+bQ_0| \cdot e^{brt}$
when $t\to \infty$, we have $|a+bQ|\to \infty$
so $|Q|\to\infty$
** 2.3
*** 6
**** a
$S(0)=0, S'-rS=k$
$P(t)=-r, Q(t)=k$
$e^{-rt}S=\int ke^{-rt} dt$
$S=-kr+Ce^{rt}$
$S=-kr+kre^{rt}$
**** b
$-k0.075+0.075ke^{0.075\times 40} \geq 100000000$
$k\geq 69801$
**** c
$-2000r+2000re^{40r} \geq 100000000$
$r\geq 50%$
*** 12
$T'=-k(T-70), T(0)=200, T(1)=190, T(?)=150$
$\frac{dT}{T-70}=-kdt$
$\ln |T-70|=-kt+C$
$T=Ce^{-kt}+70$
using $T(0)=200$, we know $C=130$
so $T=130e^{-kt}+70$
using $T(1)=190$, we know $130e^{-k}=120$
then $k=\ln 13-\ln 12$
so $T=120e^{-t}+70$
we want $150=120e^{-t}+70$
then $e^{-t}=\frac{2}{3}$
so $t=\ln 3-\ln 2$, in minutes.
*** 18
a ball with mass $0.15kg$ upward initial velocity $20m/s$ from $30m$ high
with air resistance of $\frac{v^2}{1325}$
it has downward gravity providing $10m/s^2$
$V'=-\frac{V^2}{1325}-10, V(0)=20$
$H'=V, H(0)=30$
$V'+\frac{1}{1325}V^2=-10$
don't know how to solve this $V^2$ equation
*** 24
$(1+y')^2y=k^2$
no idea how to do this when $y'^2$ exists.
