#+TITLE: 11.29math
#+AUTHOR: 2024110144

* Derivation

Since $f(x) = \frac{2x + 3}{x^2 + 3x}$ can be seen as $f(x) = \frac{1}{x} + \frac{1}{x+3}$

We know that $f^{(n)} (-2) = \sum_{k=0}^n C_n^k (-1)^n \left(\frac{1}{x^n} + \frac{1}{(x+3)^n}\right)$

* LIMITS A

Expend the function at point $x_0$ where $f(x_0) = 2$
\begin{align*}
f(x) &= 2 + \frac{f'(x_0)}{1!} (x - x_0) + \frac{f"(x_0)}{2!} (x - x_0)^2 + \frac{f^{(3)}(x_0)}{3!} (x - x_0)^3 + o(x^4)\\
&= 2 + \frac{f"(x_0)}{2!} (x - x_0)^2 + \frac{f^{(3)}(x_0)}{3!} (x - x_0)^3 + o(x^4)
\end{align*}

Assign $x = 0, 1$
\begin{align*}
0 &= 2 + \frac{f"(x_0) x_0^2}{2}\\
&= 2 + \frac{f"(x_0) (1 - x_0)^2}{2} + \frac{f^{(3)}(x_0) (1 - x_0)^3}{6}
\end{align*}

Since there must be one smaller than $0.25$ between $x_0^2$ and $(1 - x_0)^2$

We know $f"(x_0) \leq -16$

If we suppose that the statement is wrong, we have $f"(x) < -16$ true for all the numbers between $0$ and $1$

Is that possible? $-16$ is such a small number that we would get an extremely steep curve for $f'(x)$

Then the question is how to exactly prove our supposement wrong

Consider $\int_{x_0}^{x_1} f"(x) dx$

We have $f'(x_1) - f'(x_0) < -16 (x_1 - x_0)$

Furthermore, consider $\int_{x_0}^{x_1} f'(x) dx$

We have $f(x_1) - f(x_0) < - 16 (x_1 - x_0)^2$

Assign $1$ and $0$ in, the supposement is obviously wrong

Thus the statement is indeed true

* LIMITS B

We have to expand the function at point $x = 1$

\begin{align*}
f(x) &= f(1) + \frac{f'(1)}{1!} (x - 1) + \frac{f"(1)}{2!} (x - 1)^2 + \frac{f^{(3)}(1)}{3!} (x - 1)^3 + o(x^4)\\
&= f(1) + \frac{f"(1)}{2} (x - 1)^2 + \frac{f^{(3)}(1)}{3!} (x - 1)^3 + o(x^4)\\
\end{align*}

Assign $x = 1, 2$

We get
\begin{align*}
1 &= f(1) + \frac{f"(1)}{2} - \frac{f^{(3)}(1)}{3!}\\
2 &= f(1) + \frac{f"(1)}{2} + \frac{f^{(3)}(1)}{3!}
\end{align*}

Substracting the above two equations by each other, we get
\begin{equation*}
1 = \frac{f^{(3)}(1)}{3}
\end{equation*}

Applying the Darboux's Theorem, we know that the statement is true

* LIMITS C
\begin{align*}
\lim_{x \to 0} \frac{x - \sin x}{x^2 \sin x} &= \lim_{x \to 0} \frac{x - \left(x - \frac{x^3}{6} + o(x^4)\right)}{x^2 \left(x - \frac{x^3}{3!} + o(x^4)\right)}\\
&= \lim_{x \to 0} \frac{\frac{x^3}{6} + o(x^4)}{x^2 \left(x + o(x^2)\right)}\\
&= \lim_{x \to 0} \frac{\frac{x^3}{6} + o(x^4)}{x^3 + o(x^4)}\\
&= \frac{1}{6}
\end{align*}

* LIMITS D
\begin{align*}
\lim_{x \to 0} \frac{24 - 12x^2 + x^4 - 24 \cos x}{\sin^6 x} &= \lim_{x \to 0} \frac{24 - 12x^2 + x^4 - 24 + 12 x^2 - x^4 + \frac{1}{30} x^6 + o(x^7)}{\left(x + o(x^2)\right)^6}\\
&= \frac{1}{30}
\end{align*}

* LIMITS E
\begin{align*}
\lim_{x \to 0} \frac{\sin (\tan x) - \tan (\sin x)}{x \sin^3 x \tan^3 x} &= \lim_{x \to 0} \frac{x + \frac{x^3}{6} - \frac{x^5}{40} - \frac{55x^7}{1008} + o (x^8) - x - \frac{x^3}{6} + \frac{x^5}{40} + \frac{107x^7}{5040} + o(x^8)}{x^7}\\
&= \lim_{x \to 0} \frac{-\frac{x^7}{30} + o(x^4)}{x^7}\\
&= -\frac{1}{30}
\end{align*}

* LIMITS F
\begin{align*}
\lim_{x \to 0} \frac{\ln \left(1 + x + x^2\right) + \ln \left(1 - x + x^2\right)}{\sec x - \cos x} &= \lim_{x \to 0} \frac{\ln \left[(1 + x + x^2)(1 - x - x^2)\right]}{x^2}\\
&= \lim_{x \to 0} \frac{\ln \left[1 + x^2 + x^4\right]}{x^2}\\
&= \lim_{x \to 0} (1 + x^2)\\
&= 1
\end{align*}
