#+TITLE: Week 10.11 Math Homework
#+AUTHOR: 2024110144 陈有骏
#+LATEX_COMPILER: xelatex
#+LATEX_CLASS: article
#+LATEX_CLASS_OPTIONS: [a4paper,10pt]
#+LATEX_HEADER: \usepackage[margin=0.5in]{geometry}
#+LATEX_HEADER: \usepackage{xeCJK}
#+LATEX_HEADER: \usepackage{fontspec}
#+LATEX_HEADER: \usepackage{amsmath}
#+LATEX_HEADER: \setCJKmainfont{WenQuanYi Zen Hei}
#+OPTIONS: \n:t toc:nil num:nil date:nil

#+begin_comment
3.1 1-21 mod 3 (P123)
第二章复习题 18-37 mod 3 (P114)
#+end_comment

* 3.1
** 3
$6y"-y'-y=0$
suppose $y=e^{rt}$
then $6r^2-r-1=0$
we get $r=\frac{1}{2}, -\frac{1}{3}$
then $y=c_1e^{\frac{1}{2}t}+c_2e^{-\frac{1}{3}t}$
** 6
$y"-2y'-2y=0$
similarly, we have $r^2-2r-2=0$
then $r=1\pm\sqrt{3}$
so $y=c_1e^{1+\sqrt{3}}+c_2e^{1-\sqrt{3}}$
** 9
$y"+3y'=0$
there is $r^2+r=0$
giving $r=0, -1$
so $y=c_1+c_2e^{-t}$
with initial conditions, $c_1+c_2=-2$ and $-c_2=3$
then $c_1=1, c_2=-3$
so $y=1-3e^{-t}$
#+begin_src gnuplot :file 10.11-3.1-9.png :exports both
  set xrange [-10:10]
  set xlabel "X"
  set ylabel "Y"
  set title "10.11-3.1-9"

  f(x) = 1-3*exp(-x)
  
  plot f(x) title "y=1-3e^{-x}"
#+end_src

#+RESULTS:
[[file:10.11-3.1-9.png]]

it goes toward a constant ($1$) as we can see, as $t$ increases
** 12
$4r^2-1=0$
$r=\pm\frac{1}{2}$
$y=c_1e^{\frac{1}{2}t}+c_2e^{-\frac{1}{2}t}$
$\begin{aligned}
c_1e^{-1}+c_2e &= 1\\
c_1e^{-1} - c_2e &= -2
\end{aligned}$
so $c_1=-\frac{e}{2}, c_2=\frac{3}{2e}$
$y = -\frac{1}{2}e^{\frac{1}{2}t+1} + \frac{3}{2}e^{-\frac{1}{2}t-1}$
#+begin_src gnuplot :file 10.11-3.1-12.png :exports both
  set xrange [-10:10]
  set xlabel "X"
  set ylabel "Y"
  set title "10.11-3.1-12"

  f(x) = -0.5*exp(0.5*x+1) + 1.5*exp(-0.5*x-1)
  
  plot f(x) notitle
#+end_src

#+RESULTS:
[[file:10.11-3.1-12.png]]

when $t$ increases, it just goes down, in a fast-slow-fast manner.
** 15
$2r^2-3r+1=0$
$(2r-1)(r-1)=0$
so $r=1, \frac{1}{2}$
$y=c_1e^t+c_2e^{\frac{t}{2}}$
$\begin{aligned}
c_1+c_2 &= 2\\
c_1+\frac{1}{2}c_2=\frac{1}{2}
\end{aligned}$
$c_1=-1, c_2=3$
so $y=-e^t+3e^{\frac{t}{2}}$
suppose $a=e^{\frac{t}{2}} > 0$
then $y = -a^2+3a$
when $a=\frac{3}{2}$, we get max $y=\frac{9}{4}$
and when $a=3$, $y=0$ which means points $t$ of $2\ln 3$
** 18
$r^2+(3-\alpha)r-2(\alpha-1)=0$
$(r+2)(r+1-\alpha)=0$
$r=-2, \alpha-1$
$y=c_1e^{-2t}+c_2e^{(\alpha-1)t}$
for the first situation, $\alpha\leq 1$ works
for the second situation, there is no such $\alpha$ that suits all
** 21
$ar^2+br+c=0$
$\Delta = b^2-4ac$
*** a
$b^2-4ac>0$
$-b+\sqrt{b^2-4ac}<0$
*** b
$b^2-4ac>0$
$c<0$
*** c
$b^2-4ac>0$
$-b-\sqrt{b^2-4ac}>0$
* review
** 18
$\frac{dy}{dx} + \frac{2y^2+6xy-4}{3x^2+4xy+3y^2} = 0$
rearrange the equation, $(2y^2+6xy-4)dx + (3x^2+4xy+3y^2)dy = 0$
check $\frac{\delta (2y^2+6xy-4)}{\delta y} = 4y+6x$
and $\frac{\delta (3x^2+4xy+3y^2)}{\delta x} = 6x+4y$
they are equal so we suppose $u(x,y)$ meeting
$$\begin{aligned}
\frac{\delta u(x,y)}{\delta x} &= 2y^2+6xy-4\\
\frac{\delta u(x,y)}{\delta y} &= 3x^2+4xy+3y^2
\end{aligned}$$
so $u(x,y)=2xy^2+3x^2y-4x+y^3+C$

** 21
$\frac{dy}{dx} = \frac{x}{x^2y+y^3}$
let $u=x^2$
$(uy+y^3)dy = \frac{1}{2}du$
$(u+y^2)d(y^2) = du$
let $v=y^2$
$(u+v)dv = du$
$u+v = \frac{du}{dv}$
$\frac{du}{dv} - u = v$
$e^{-v}\frac{du}{dv} - e^{-v} u = v$
$\frac{de^{-v}u}{dv} = v$
$e^{-v}u = \frac{1}{2} v^2 + C$
$u = \frac{1}{2} v^2 e^v + C$
$x^2 = \frac{1}{2} y^4 e^{y^2} + C$

** 24
$xy'+y-y^2e^{2x}=0, y(1)=2$
$xdy + (y-y^2e^{2x}) dx=0$
when $y=0, xy'=0$
when $x=0, y=y^2$
when $x, y\neq 0$, $\frac{x}{y^2}dy + (\frac{1}{y}-e^{2x})dx = 0$
I want $\frac{x^{n+1}}{y^2}dy + (\frac{x^n}{y} - x^ne^{2x})dx = 0$
where $(n+1)\frac{x^n}{y^2}=-\frac{x^n}{y^2}-0$
giving $n=-2$
so $\frac{1}{xy^2}dy + \left(\frac{1}{x^2y} - \frac{e^{2x}}{x^2}\right)dx = 0$
we need $u(x, y) = -\frac{1}{xy} - \int \frac{e^{2x}}{x^2} dx + C$
don't know the solution of the integral embedded
** 27
*** a
$\frac{dy}{dt} = (1-y)(x(t)+by)$
$y'=-by^2+(b-x(t))y+x(t)$
so it is a Ribbeca equation
apply $y_1(t)=1$
we get $0=-b+b-x(t)+x(t)$, true
let $y=y_1(t)+\frac{1}{v(t)}$ so $y=1+\frac{1}{v(t)}$
then $-\frac{v'(t)}{v^2(t)} = -b(1+\frac{1}{v(t)})^2+(b-x(t))(1+\frac{1}{v(t)})+x(t)$
$\frac{dv}{dt} = (b+x(t))v+b$
*** b
$\frac{dv}{dt} = (b+at)v+b$
$v'-(b+at)v = b$
$e^{-bt-\frac{a}{2}t^2}v=bt+C$
$v=bte^{bt+\frac{a}{2}t^2} + C$
** 30
$y"+ty'^2=0$
$v'+tv^2=0$
$dv + tv^2 dt=0$
$2dv + v^2 d(t^2) = 0$
suppose $n = t^2$, $2dv + v^2 dn = 0$
then $\frac{2}{v^2} dv + dn = 0$
we get $u(v,n)=-\frac{2v}{v^2}+n+C$
so $-\frac{2}{v^2} + t^2 = C$
$\frac{2}{v^2} = t^2-C$
$v^2=\frac{2}{t^2-C}$
$v=\pm \sqrt{\frac{2}{t^2-C}}$
$y = \pm \int \sqrt{\frac{2}{t^2-C}} dt$
** 33
$y"+y=0$
suppose $v=y'$
then $y"=v\cdot\frac{dv}{dy}$
$\frac{vdv}{dy}+y=0$
$vdv+ydy=0$
$\frac{1}{2}v^2+\frac{1}{2}y^2+C=0$
$v^2+y^2=0$
$y=0$
** 36
$y'y"=2, y(0)=1, y'(0)=2$
$vv'=2$
$vdv-2dy=0$
$\frac{1}{2}v^2-2y+C=0$
$v^2-4y=C$
$y'^2-4y=C$
$C=0$
$y'^2=4y$
we can see $y=t^2$ is an answer
don't know if other answers exists
