#+TITLE: Week 10.13 Math Homework
#+AUTHOR: 2024110144 陈有骏
#+LATEX_COMPILER: xelatex
#+LATEX_CLASS: article
#+LATEX_CLASS_OPTIONS: [a4paper,10pt]
#+LATEX_HEADER: \usepackage[margin=0.5in]{geometry}
#+LATEX_HEADER: \usepackage{xeCJK}
#+LATEX_HEADER: \usepackage{fontspec}
#+LATEX_HEADER: \usepackage{amsmath}
#+LATEX_HEADER: \setCJKmainfont{WenQuanYi Zen Hei}
#+OPTIONS: \n:t toc:nil num:nil date:nil

#+begin_comment
3.2 1-38 mod 5 (P133)
3.3 1-36 mod 5 (P139)
3.4 1-30 mod 6 (P147)
#+end_comment

* 3.2
** 5
$cos^2\theta, 1 + \cos (2\theta)$
$\begin{aligned}
W
&= \left|\begin{matrix}
\cos^2\theta & 1+\cos(2\theta)\\
(\cos^2\theta)' & (1+\cos(2\theta))'
\end{matrix}\right|\\
&= \left|\begin{matrix}
\cos^2\theta & 1+\cos(2\theta)\\
-2\cos\theta\sin\theta & -2\sin(2\theta)
\end{matrix}\right|\\
&= \left|\begin{matrix}
\cos^2\theta & 1+\cos(2\theta)\\
-\sin(2\theta) & -2\sin(2\theta)
\end{matrix}\right|\\
&= -2\sin(2\theta)\cos^2\theta + (1+\cos(2\theta))\sin(2\theta)\\
&= \sin(2\theta) (1+\cos(2\theta)-2\cos^2\theta)\\
&= \sin(2\theta) (1+\cos^2\theta-\sin^2\theta-2\cos^2\theta)\\
&= \sin(2\theta) \cdot 0\\
&= 0
\end{aligned}$

** 10
apply $y_1(t)=t^2$
we get $2t^2-2t^2=0$
apply $y_2(t)=t^{-1}$
we get $\frac{2}{t}-2\cdot \frac{1}{t}=0$
apply $y = c_1t^2+c_2t^{-1}$
since $y'' = 2c_1+2c_2\cdot t^{-3}$
we get $2c_1t^2+2c_2\cdot t^{-1} - 2c_1t^2 - 2c_2\cdot t^{-1} = 0$

** 15
$W[f, g] = fg' - gf' = t\cos t-\sin t$
here $u = f + 3g, v = f - g$
$\begin{aligned}
W[u, v]
&= uv' - vu'\\
&= (f+3g)(f'-g') - (f-g)(f'+3g')\\
&= ff'-fg'+3f'g-3gg'-ff'-3fg'+gf'+3gg'\\
&= 4(gf'-fg')\\
&= -4t\cos t + 4\sin t
\end{aligned}$

** 20
apply $y_1(t)=e^t$
we get $e^t-2e^t+e^t=0$
apply $y_2(t)=te^t$
we get $(t+2)e^t-2(t+1)e^t+te^t=0$
check $\begin{aligned}
W[y_1, y_2]
&= e^t(t+1)e^t - te^te^t\\
&= e^{2t}
\end{aligned}$
not zero, so does constitute a fundamental set of solutions

** 25

** 30
#+begin_comment
Prove that if $y_1$ and $y_2$ have a common point of inflection $t_0$ in $I$
then they cannot be a fundamental set of solutions on $I$ unless both $p$ and $q$
are zero at $t_0$
#+end_comment
$y''+p(t)y'+q(t)y=0, y_1''(t_0)=y_2''(t_0)=0$
$W[y_1, y_2] = y_1y_2'-y_1'y_2$
$p(t_0)y_1'+q(t_0)y_1=0, p(t_0)y_2'+q(t_0)y_2=0$
they are a fundamental set of solutions only when $y_1y_2'=y_1'y_2$
if $p(t_0)\neq 0, q(t_0)\neq 0$
since they have inflection point, they can't be zero
so $\frac{y_1}{y_1'}=\frac{y_2}{y_2'}=\frac{y_1\pm y_2}{y_1'\pm y_2'}=-\frac{p(t_0)}{q(t_0)}$
then $y_1=ky_2, y_1'=ky_2'$
impossible
if $p(t_0)\neq 0, q(t_0)=0$
$y_1'=y_2'=0$
since $y_1''=y_2''=0$, we have $y_1=C_1, y_2=C_2$
impossible
if $p(t_0)=0, q(t_0)\neq 0$
$y_1=y_2=0$
since $y_1''=y_2''=0$, we know $y_1, y_2$ one forever $\geq 0$, the other forever $\leq 0$
impossible
so only when $y_1\neq 0, y_2\neq 0$
$\frac{y_1}{y_1'}=\frac{y_2}{y_2'}=-\frac{p(t_0)}{q(t_0)}$
$y_1y_2'-y_1'y_2 = 0$
true

** 35

* 3.3
** 5
$y''-2y'+2y=0$
$r^2-2r+2=0$
$r=\frac{2\pm 2i}{2}=1\pm i$
$y=c_1e^{(1+i)t}+c_2e^{(1-i)t}=e^t(c_1e^{-it}+c_2e^{it})$
$y=e^t(c_1\cos(-t)+c_1i\sin(-t)+c_2\cos t+c_2i\sin t$
$y=e^t(C_1\cos t + iC_2\sin t)$
** 10
$9y''+9y'-4y=0$
$r=\frac{-9\pm 15}{18}=-\frac{1}{2}\pm \frac{5}{6}$
$r=\frac{1}{3}, -\frac{4}{3}$
$y=c_1e^{\frac{1}{3}t}+c_2e^{-\frac{4}{3}t}$
** 15
$y''+2y'+2y=0, y(\frac{\pi}{4})=2, y'(\frac{\pi}{4})=-2$
$r=-1\pm i$
$y=e^{-t}(C_1\cos t + iC_2\sin t)$
$\begin{aligned}
y'
&= -e^{-t}(C_1\cos t + iC_2\sin t)+e^{-t}(-C_1\sin t+iC_2\cos t)\\
&= e^{-t}\left((-C_1-iC_2)\sin t+(-C_1+iC_2)\cos t\right)
\end{aligned}$
apply initial conditions
we get $e^{-\frac{\pi}{4}}\cdot \frac{\sqrt{2}}{2} \cdot (C_1+iC_2)=2$
and $e^{-\frac{\pi}{4}}\cdot \frac{\sqrt{2}}{2} \cdot (-2C_1)=-2$
so $\begin{aligned}
C_1+iC_2 &= 2\sqrt{2} e^{\frac{\pi}{4}}\\
2C_1 &= -2\sqrt{2} e^{\frac{\pi}{4}}
\end{aligned}$
this gives $\left{\begin{aligned}
C_1 &= -\sqrt{2} e^{\frac{\pi}{4}}\\
C_2 &= -i \cdot 3\sqrt{2} e^{\frac{\pi}{4}}
\end{aligned}\right .$
$y = -\sqrt{2}e^{-t+\frac{\pi}{4}}(\cos t - 3\sin t)$

#+begin_src gnuplot :file 10.13-3.3-15.png :exports both
  set term png size 300,300
  set xlabel "t"
  set ylabel "y"

  f(x)=-sqrt(2)*exp(-x+pi/4.0)*(cos(x)-3*sin(x))

  plot f(x) notitle
#+end_src

#+RESULTS:
[[file:10.13-3.3-15.png]]

when $t$ increases, $y$ first goes down, then up, at last approachs $0$

** 20
*** a
$y''+y=0$
apply $y_1(t)=\cos t$
we get $-\cos t+\cos t=0$
apply $y_2(t)=\sin t$
we get $-\sin t+\sin t=0$
since $\begin{aligned}
W[y_1, y_2]
&= y_1y_2' - y_1'y_2\\
&= \cos t \cos t + \sin t \sin t\\
&= 1
\end{aligned}$
*** b
apply $y=e^{it}$
we get $i\cdot ie^{it} + e^{it}=0$
and since $y_1, y_2$ is fundamental, $e^{it}=c_1y_1+c_2y_2$
*** c
when $t=0$, we have $1=c_1+0$
*** d
$ie^{it} = -c_1\sin t + c_2\cos t$
when $t=0$, we have $i=-0+c_2$
with $c$, we have $e^{it}=\cos t + i\sin t$
let $\theta = t$, it is Euler's Formula
** 25
*** a
$\frac{dy}{dt} = \frac{dy}{dx}\cdot\frac{dx}{dt} = \frac{1}{t}\cdot\frac{dy}{dx}$
$\begin{aligned}
\frac{d^2y}{dt^2}
&= -\frac{1}{t^2} \cdot \frac{dy}{dx} + \frac{1}{t}\cdot \frac{d^2y}{dxdt}\\
&= -\frac{1}{t^2} \cdot \frac{dy}{dx} + \frac{1}{t^2}\cdot \frac{d^2y}{dx^2}
\end{aligned}$
*** b
apply results in $a$
we get $- \frac{dy}{dx} + \frac{d^2y}{dx^2} + \alpha \frac{dy}{dx} + \beta y = 0$
which is just $\frac{d^2y}{dx^2} + (\alpha-1) \frac{dy}{dx} + \beta y = 0$
** 30
$x=\ln t$
$\frac{d^2y}{dx^2} + 2\frac{dy}{dx} - 3y = 0$
$y''+2y'-3y=0$
$r^2+2r-3=0$
$(r+3)(r-1)=0$
$r=-3, 1$
$y_1(x)=e^{-3x}, y_2(x)=e^x$
$\begin{aligned}
W[y_1, y_2]
&= \left|\begin{matrix}
e^{-3x} & e^x\\
-3e^{-3x} & e^x
\end{matrix}\right|\\
&= e^{-2x}\left(1\times 1 - 1\times (-3)\right) \neq 0$
so $y_1(x)$ and $y_2(x)$ form a fundamental set of solution
then $y_1(\ln t), y_2(\ln t)$ form as well
so $y=c_1\frac{1}{t^3} + c_2t$
** 35
since $t>0$, $y''+(t-\frac{1}{t})y'+t^2y=0$
$x=u(t), p(t)=t-\frac{1}{t}, q(t)=t^2$
here $q(t)=t^2>0, 0<t<\infty$
so $x = u(t) = \int t dt = \frac{1}{2} t^2 + C$
since $\left(\frac{dx}{dt}\right)^2 = t^2$
then $frac{d^2x}{dt^2}=1$ and $p(t)\frac{dx}{dt}=(t^2-1)$
we have $t^2\frac{d^2y}{dx^2} + (1+t^2-1)\frac{dy}{dx} + t^2y = 0$
since $t^2>0$, we get $\frac{d^2y}{dx^2} + \frac{dy}{dx} + y = 0$
from $r^2+r+1=0$ we have $r=\frac{-1\pm i\sqrt{3}}{2}$
so $y_1(x)=e^{\frac{-1+i\sqrt{3}}{2}\cdot x}, y_2(x)=e^{\frac{-1-i\sqrt{3}}{2}\cdot x}$
$\begin{aligned}
W[y_1, y_2]
&= \left|\begin{matrix}
y_1(x) & y_2(x)\\
\frac{-1+i\sqrt{3}}{2}y_1(x) & \frac{-1-i\sqrt{3}}{2}y_2(x)
\end{matrix}\right|\\
&= \left|\begin{matrix}
e^{\frac{-1+i\sqrt{3}}{2}\cdot x} & e^{\frac{-1-i\sqrt{3}}{2}\cdot x}\\
\frac{-1+i\sqrt{3}}{2}e^{\frac{-1+i\sqrt{3}}{2}\cdot x} & \frac{-1-i\sqrt{3}}{2}e^{\frac{-1-i\sqrt{3}}{2}\cdot x}
\end{matrix}\right|\\
&= \frac{-1-i\sqrt{3}}{2}e^{-x} - \frac{-1+i\sqrt{3}}{2}e^{-x}\\
&= e^{-x}\left(\frac{-1-i\sqrt{3}}{2}-\frac{-1+i\sqrt{3}}{2}\right)\\
&= -e^{-x}\\
&\neq 0
\end{aligned}$
so $y_1(x), y_2(x)$ is a fundamental set of solution
then $y_1(\frac{1}{2} t^2 + C), y_2(\frac{1}{2} t^2 + C)$ is as well
which means $\begin{aligned}
y &= c_1e^{\frac{-1+i\sqrt{3}}{2}\cdot (\frac{1}{2} t^2 + C)} + c_2e^{\frac{-1-i\sqrt{3}}{2}\cdot (\frac{1}{2} t^2 + C)}\\
&= c_1e^{\frac{-1+i\sqrt{3}}{2}\cdot \frac{1}{2} t^2} + c_2e^{\frac{-1-i\sqrt{3}}{2}\cdot \frac{1}{2} t^2}\\
&= c_1e^{\frac{-1+i\sqrt{3}}{4} t^2} + c_2e^{\frac{-1-i\sqrt{3}}{4} t^2}
\end{aligned}$

* 3.4
** 6
$4y''+17y'+4y=0$
$4r^2+17r+4=0$
$\Delta = 17^2 - 4\times 4\times 4 = 225 = 15^2$
$r = \frac{-17\pm 15}{8}$
$r = -\frac{1}{4}, -4$
$y = c_1e^{-\frac{t}{4}}+c_2e^{-4t}$
** 12
$r=\frac{1}{2}$
$y=(c_1+c_2t)e^{\frac{t}{2}}$
apply $y(0)=2$
we get $c_1=2$
so $y=(2+c_2t)e^{\frac{t}{2}}$
apply $y'(0)=b$
since $y' = (\frac{c_1+c_2t}{2}+c_2)e^{\frac{t}{2}}$
we get $c_2+1=b$
so $y=(2+(b-1)t)e^{\frac{t}{2}}$
the critical point is of course $b=1$
** 18
since $t>0$, $y''-\frac{4}{t}y'+\frac{6}{t^2}y=0$
$p(t)=-\frac{4}{t}, q(t)=\frac{6}{t^2}$
given $y_1(t)=t^2$
we suppose $y=v(t)y_1(t)=v(t)t^2$
then $y'=v'(t)t^2+2tv(t)$
$y''=v''(t)t^2+4tv'(t)+2v(t)$
$v''(t)t^2+4tv'(t)+2v(t)+p(t)v'(t)t^2+2tp(t)v(t)+q(t)y=0$
$v''(t)t^2+4tv'(t)
** 24
** 30
