#+TITLE: Week 4.14 Math Homework
#+AUTHOR: 2024110144 陈有骏
#+LATEX_COMPILER: xelatex
#+LATEX_CLASS: article
#+LATEX_CLASS_OPTIONS: [a4paper,10pt]
#+LATEX_HEADER: \usepackage[margin=0.5in]{geometry}
#+LATEX_HEADER: \usepackage{xeCJK}
#+OPTIONS: \n:t toc:nil num:nil date:nil

#+begin_comment
4.14
导论 下 7.2 1,2,3中奇数小题
2 1
3 9
#+end_comment

* some additional
** $xyz \rightarrow zr\theta$
$r\cos\theta \, r\sin\theta \, z$

| 0              | 0               | 1 |
| $\cos\theta$   | $\sin\theta 0$  | 0 |
| $-r\sin\theta$ | $r\cos\theta 0$ | 0 |

the jacobbi determant equals to $r$
** $xyz \rightarrow \phi\rho\theta$
for simplicity, we require $\rho \in (-\frac{\pi}{2},\frac{\pi}{2})$
so $xyz$ is $\rho \cos \phi \cos \theta \, \rho \cos \phi \sin \theta \, \rho \sin \phi$

| \cos \phi \cos \theta        | \cos \phi \sin \theta        | \sin \phi      |
| - \rho \sin \phi \cos \theta | - \rho \sin \phi \sin \theta | \rho \cos \phi |
| - \rho \cos \phi \sin \theta | \rho \cos \phi \cos \theta   | 0              |

$$\begin{align*}
J &= 0 - \rho^2 (\cos^3 \phi \sin^2 \theta + \sin^2 \phi \cos \phi \cos^2 \theta)\\
&\quad - \rho^2 \sin^2 \phi \cos \phi \sin^2 \theta - \rho^2 \cos^3 \phi \cos^2 \theta\\
&= - \rho^2 (\cos^3 \phi + \sin^2 \phi \cos \phi)\\
&= - \rho^2 (\sin\phi + \cos\phi)
\end{align*}$$
so we need to multiply $\rho^2 |\sin\phi+\cos\phi|$

* 4.14
** 1
*** 1
$$\iiint_V xydxdydz$$
$$V:1\leq x\leq 2,\,-2\leq y\leq 1,\,0\leq z\leq \frac{1}{2}$$
because $xy$ is continuous in $\mathbb{R}^3$
we can use triple integral to calculate
note that $y$ crosses $0$ but volumn should always be non-negative
we should add $y$ for $[-2,0],[0,1]$ separately
$$\begin{align*}
\iiint_V xydxdydz
&= \int_0^{\frac{1}{2}} (\int_{-2}^1)_{special} \int_1^2 xy dxdydz\\
&= \int_0^{\frac{1}{2}} (\int_{-2}^1)_{special} \frac{x^2y}{2} |_1^2 dydz\\
&= \int_0^{\frac{1}{2}} (\int_{-2}^1)_{special} \frac{3y}{2} dydz\\
&= \frac{3}{2} \int_0^{\frac{1}{2}} (\int_{-2}^1)_{special} y dydz\\
&= \frac{3}{2} \int_0^{\frac{1}{2}} \frac{y^2}{2} (|_{-2}^1)_{special} dz\\
&= \frac{3}{2} \int_0^{\frac{1}{2}} \frac{5}{2} dz\\
&= \frac{15}{4} \int_0^{\frac{1}{2}} dz\\
&= \frac{15}{4} \cdot \frac{1}{2}\\
&= \frac{15}{8}
\end{align*}$$
*** 3
$$\iiint_V xy^2z^3dxdydz$$
$$V:\text{由}z=xy,y=x,x=1,z=0\text{围成}$$
$$\begin{align*}
\iiint_V xy^2z^3dxdydz
&= \int_0^1 \int_0^x \int_0^{xy} xy^2z^3 dzdydx\\
&= \int_0^1 \int_0^x \frac{xy^2z^4}{4} |_0^{xy} dydx\\
&= \int_0^1 \int_0^x \frac{x^5y^6}{4} dydx\\
&= \int_0^1 \frac{x^5y^7}{28} |_0^x dx\\
&= \int_0^1 \frac{x^12}{28} dx\\
&= \frac{x^13}{28\times 13} |_0^1\\
&= \frac{1}{28\times 13}\\
&= \frac{1}{364}
\end{align*}$$
#+begin_src scheme :exports both
  (* 28 13)
#+end_src

#+RESULTS:
: 364

*** 5
$$\iiint_V (x+y) dxdydz$$
$$V:\text{由}z=1-x^2-y^2,z=0\text{围成}$$
we can see this as $z=1-r^2,z=0$
and $\iiint_V r(\cos\theta + \sin\theta) r dzdrd\theta$
$$\begin{align*}
\iiint_V r(\cos\theta + \sin\theta) dzdrd\theta
&= \int_0^{2\pi} \int_0^1 \int_0^{1-r^2} r^2 (\cos\theta + \sin\theta) dzdrd\theta\\
&= \int_0^{2\pi} \int_0^1 (1-r^2)r^2(\cos\theta + \sin\theta) drd\theta\\
&= \int_0^{2\pi} \int_0^1 (r^2-r^4)(\cos\theta + \sin\theta) drd\theta\\
&= \int_0^{2\pi} (\frac{r^3}{3}-\frac{r^5}{5})|_0^1 (\cos\theta + \sin\theta) d\theta\\
&= \int_0^{2\pi} \frac{2}{15} (\cos\theta + \sin\theta) d\theta\\
&= \frac{2}{15} \int_0^{2\pi} (\cos\theta + \sin\theta) d\theta\\
&= \frac{2}{15} (\sin\theta - \cos\theta)|_0^{2\pi}\\
&= \frac{2}{15} \cdot 0\\
&= 0
\end{align*}$$
** 2
*** 1
$$\begin{align*}
&r\cos \theta &\in [0,2]\\
&r\sin \theta &\in [0,\sqrt{2r\cos\theta - r^2\cos^2\theta}]
\end{align*}$$
$$\begin{align*}
\int_0^2 dx \int_0^{\sqrt{2x-x^2}} dy int_0^a z\sqrt{x^2+y^2} dz
&= \int_0^2 dx \int_0^{\sqrt{2x-x^2}} dy \frac{z^2}{2} \sqrt{x^2+y^2} |_0^a\\
&= \int_0^2 dx \int_0^{\sqrt{2x-x^2}} dy \frac{a^2}{2} \sqrt{x^2+y^2}\\
&= \frac{a^2}{2} \int_0^2 dx \int_0^{\sqrt{2x-x^2}} dy \sqrt{x^2+y^2}\\
&= \frac{a^2}{2} \int_0^2 dx \int_0^{\sqrt{2x-x^2}} \sqrt{x^2+y^2} dy\\
&= \frac{a^2}{2} \int_0^2 dr \int_0^{\sqrt{2x-x^2}} r^2 d\theta\\
\end{align*}$$
*** 3
$$\begin{align*}
\int_0^1 dx \int_0^{\sqrt{1-x^2}} dy \int_0^{\sqrt{1-x^2-y^2}} \sqrt{x^2+y^2+z^2} dz
&= \iiint_{V:x^2+y^2+z^2\leq 1} \sqrt{x^2+y^2+z^2} dA\\
&= \iiint_{V:\rho^2 \leq 1} \rho dA\\
&= \int_0^{2\pi} \int_0^{\pi} \int_0^1 \rho d\rho d\phi d\theta\\
&= \int_0^{2\pi} \int_0^{\pi} \frac{\rho^2}{2} |_0^1 d\phi d\theta\\
&= \int_0^{2\pi} \int_0^{\pi} \frac{1}{2} d\phi d\theta\\
&= 2\pi^2 \cdot \frac{1}{2}\\
&= \pi^2
\end{align*}$$
** 3
*** 1
$$\iiint_V (x^2+y^2) dxdydz$$
$$V:\text{由}x^2+y^2=2z,z=2\text{围成}$$
we can use $x^2+y^2=r^2$
so
$$\begin{align*}
\iiint_V (x^2+y^2) dxdydz
&= \iiint_V r^2 dzdrd\theta\\
&= \int_0^{2\pi} \int_0^2 \int_{\frac{r^2}{2}}^2 r^2 dzdrd\theta\\
&= \int_0^{2\pi} \int_0^2 (2-\frac{r^2}{2})r^2 drd\theta\\
&= \int_0^{2\pi} \int_0^2 (2r^2-\frac{r^4}{2}) drd\theta\\
&= \int_0^{2\pi} (\frac{2r^3}{3}-\frac{r^5}{10}) |_0^2 d\theta\\
&= \int_0^{2\pi} (\frac{16}{3}-\frac{16}{5}) d\theta\\
&= \frac{32\pi}{3}-\frac{32\pi}{5}\\
&= \frac{64\pi}{15}
\end{align*}$$
*** 3
$$\iiint_V xdxdydz$$
$$V:\text{由}x^2+y^2=z^2,x^2+y^2=1\text{围成}$$
we have $r^2=z^2,r^2=1$
the volumn is very special since it is like a triangle spinning around the z-axis
so
$$\begin{align*}
\iiint_V xdxdydz
&= 2 \int_0^{2\pi} \int_0^1 \int_z^1 r^2 \cos \theta drdzd\theta\\
&= 2 \int_0^{2\pi} \int_0^1 \frac{r^3}{3} \cos \theta |_0^z dzd\theta\\
&= 2 \int_0^{2\pi} \int_0^1 \frac{z^3}{3} \cos \theta dzd\theta\\
&= \int_0^{2\pi} \frac{z^4}{6} \cos \theta |_0^1 d\theta\\
&= \int_0^{2\pi} \frac{1}{6} \cos \theta d\theta\\
&= \frac{1}{6} \sin \theta |_0^{2\pi}\\
&= \frac{1}{6} \cdot 0\\
&= 0
\end{align*}$$
*** 5
$$\iiint_V z dxdydz$$
$$V:\text{由}z=\sqrt{4-x^2-y^2},x^2+y^2=3z\text{围成}$$
since $z$ is continuous, we can change the order
$z=\sqrt{4-r^2},z=\frac{r^2}{3}$
when changed to $r,\theta,z$
the ranges becom $(0,2),(0,2\pi),(\sqrt{4-r^2},\frac{r^2}{3})$
$$\begin{align*}
\iiint_V z dxdydz
&= \int_{-2}^2 \int_{-\sqrt{4-x^2}}^{\sqrt{4-x^2}} \int_{\sqrt{4-x^2-y^2}}^{\frac{x^2+y^2}{3}} z dxdydz\\
&= \int_0^{2\pi} \int_0^2 \int_{\sqrt{4-r^2}}^{\frac{r^2}{3}} zr dzdrd\theta\\
&= \int_0^{2\pi} \int_0^2 \frac{z^2}{2} |_{\sqrt{4-r^2}}^{\frac{r^2}{3}} rdrd\theta\\
&= \frac{1}{2} \int_0^{2\pi} \int_0^2 z^2 |_{\sqrt{4-r^2}}^{\frac{r^2}{3}} rdrd\theta\\
&= \frac{1}{2} \int_0^{2\pi} \int_0^2 \frac{r^5}{9}-(4r-r^3) drd\theta\\
&= \frac{1}{2} \int_0^{2\pi} \frac{r^6}{54}-2r^2+\frac{r^4}{4} |_0^2 d\theta\\
&= \frac{1}{2} \int_0^{2\pi} \frac{32}{27}-8+4 d\theta\\
&= \pi \cdot \left(\frac{32}{27}-4\right)\\
&= -\frac{76\pi}{27}
\end{align*}$$
#+begin_src scheme :exports both
  (- 32/27 4)
#+end_src

#+RESULTS:
: -76/27

*** 7
$$\iiint_V \left| x^2+y^2+z^2-1 \right| dxdydz$$
$$V:\text{由}x^2+y^2+z^2\leq 4\text{围成}$$
we shall change this to $\rho,\phi,\theta$ system
where $\rho \in [0,2]$
$$\begin{align*}
\iiint_V \left| x^2+y^2+z^2-1 \right| dxdydz
&= \iiint_{V'} \left| \rho^2 - 1 \right| \rho^2 |\sin\phi+\cos\phi| d\rho d\phi d\theta\\
&= \int_0^{2\pi} \int_{-\frac{\pi}{2}}^{\frac{\pi}{2}} \int_0^2 \left| \rho^2 - 1 \right| \rho^2 |\sin\phi+\cos\phi| d\rho d\phi d\theta\\
&= \int_0^{2\pi} \int_{-\frac{\pi}{2}}^{\frac{\pi}{2}} |\sin\phi+\cos\phi| \int_0^2 \left| \rho^2 - 1 \right| \rho^2 d\rho d\phi d\theta\\
&= \int_0^{2\pi} \int_{-\frac{\pi}{2}}^{\frac{\pi}{2}} |\sin\phi+\cos\phi| \left(\int_0^1 \left(1 - \rho^2\right) \rho^2 + \int_1^2 \left(\rho^2 - 1\right) \rho^2\right) d\rho d\phi d\theta\\
&= \int_0^{2\pi} \int_{-\frac{\pi}{2}}^{\frac{\pi}{2}} |\sin\phi+\cos\phi| \left(\int_0^1 \rho^2 - \rho^4 + \int_1^2 \rho^4 - \rho^2\right) d\rho d\phi d\theta\\
&= \int_0^{2\pi} \int_{-\frac{\pi}{2}}^{\frac{\pi}{2}} |\sin\phi+\cos\phi| \left(\int_0^1 \rho^2 - \rho^4 d\rho + \int_1^2 \rho^4 - \rho^2 d\rho\right) d\phi d\theta\\
&= \int_0^{2\pi} \int_{-\frac{\pi}{2}}^{\frac{\pi}{2}} |\sin\phi+\cos\phi| \left(\frac{\rho^3}{3} - \frac{\rho^5}{5} |_0^1 + \frac{\rho^5}{5} - \frac{\rho^3}{3} |_1^2\right) d\phi d\theta\\
&= \int_0^{2\pi} \int_{-\frac{\pi}{2}}^{\frac{\pi}{2}} |\sin\phi+\cos\phi| \left(\frac{1}{3} - \frac{1}{5} + \frac{31}{5} - \frac{7}{3}\right) d\phi d\theta\\
&= \int_0^{2\pi} \int_{-\frac{\pi}{2}}^{\frac{\pi}{2}} |\sin\phi+\cos\phi| \left(6 - 2\right) d\phi d\theta\\
&= \int_0^{2\pi} \int_{-\frac{\pi}{2}}^{\frac{\pi}{2}} |\sin\phi+\cos\phi| \cdot 4 d\phi d\theta\\
&= 4 \int_0^{2\pi} \int_{-\frac{\pi}{2}}^{\frac{\pi}{2}} |\sin\phi+\cos\phi| d\phi d\theta\\
&= 4 \int_0^{2\pi} \left(\int_{-\frac{\pi}{2}}^{-\frac{\pi}{4}} -(\sin\phi+\cos\phi) d\phi + \int_{-\frac{\pi}{4}}^{\frac{\pi}{2}} (\sin\phi + \cos\phi) d\phi\right) d\theta\\
&= 4 \int_0^{2\pi} \left(\int_{-\frac{\pi}{4}}^{-\frac{\pi}{2}} (\sin\phi+\cos\phi) d\phi + \int_{-\frac{\pi}{4}}^{\frac{\pi}{2}} (\sin\phi + \cos\phi) d\phi\right) d\theta\\
&= 4 \int_0^{2\pi} \left((\sin\phi-\cos\phi) |_{-\frac{\pi}{4}}^{-\frac{\pi}{2}} + (\sin\phi - \cos\phi) |_{-\frac{\pi}{4}}^{\frac{\pi}{2}}\right) d\theta\\
&= 4 \int_0^{2\pi} \left((-1+\frac{\sqrt{2}}{2}-\frac{\sqrt{2}}{2}) + (1-\frac{\sqrt{2}}{2} - \frac{\sqrt{2}}{2})\right) d\theta\\
&= -4\sqrt{2} \int_0^{2\pi} d\theta\\
&= -8\sqrt{2}\pi
\end{align*}$$
*** 9
$$\iiint_V \frac{z\ln(x^2+y^2+z^2+1)}{x^2+y^2+z^2+1} dxdydz$$
$$V:\text{由}x^2+y^2+z^2\leq 1\text{围成}$$
it is continuous, so we can change the system
$$\begin{align*}
\iiint_V \frac{z\ln(x^2+y^2+z^2+1)}{x^2+y^2+z^2+1} dxdydz
&= \int_0^{2\pi} \int_{-\frac{\pi}{2}}^{\frac{\pi}{2}} \int_0^1 \frac{\rho\sin\phi \ln (\rho^2+1)}{\rho^2+1} d\rho d\phi d\theta\\
&= \frac{1}{2} \int_0^{2\pi} \int_{-\frac{\pi}{2}}^{\frac{\pi}{2}} \int_0^1 \frac{\sin\phi \ln (\rho^2+1)}{\rho^2+1} d\rho^2 d\phi d\theta\\
&= \frac{1}{2} \int_0^{2\pi} \int_{-\frac{\pi}{2}}^{\frac{\pi}{2}} \int_0^1 \frac{\sin\phi \ln (\rho+1)}{\rho+1} d\rho d\phi d\theta\\
&= \frac{1}{2} \int_0^{2\pi} \int_{-\frac{\pi}{2}}^{\frac{\pi}{2}} \int_0^1 \frac{\sin\phi \ln (\rho+1)}{\rho+1} d(\rho+1) d\phi d\theta\\
&= \frac{1}{2} \int_0^{2\pi} \int_{-\frac{\pi}{2}}^{\frac{\pi}{2}} \int_1^2 \frac{\sin\phi \ln \rho}{\rho} d\rho d\phi d\theta\\
&= \frac{1}{2} \int_0^{2\pi} \int_{-\frac{\pi}{2}}^{\frac{\pi}{2}} \int_1^2 \sin\phi \ln \rho d\ln\rho d\phi d\theta\\
&= \frac{1}{2} \int_0^{2\pi} \int_{-\frac{\pi}{2}}^{\frac{\pi}{2}} \int_0^{\ln 2} \sin\phi \rho d\rho d\phi d\theta\\
&= \frac{1}{4} \int_0^{2\pi} \int_{-\frac{\pi}{2}}^{\frac{\pi}{2}} \sin\phi \rho^2 |_0^{\ln 2} d\phi d\theta\\
&= \frac{1}{4} \int_0^{2\pi} \int_{-\frac{\pi}{2}}^{\frac{\pi}{2}} \sin\phi \ln^2 2 d\phi d\theta\\
&= \frac{\ln^2 2}{4} \int_0^{2\pi} \int_{-\frac{\pi}{2}}^{\frac{\pi}{2}} \sin\phi d\phi d\theta\\
&= -\frac{\ln^2 2}{4} \int_0^{2\pi} \cos\phi |_{-\frac{\pi}{2}}^{\frac{\pi}{2}} d\theta\\
&= -\frac{\ln^2 2}{4} \int_0^{2\pi} \cos\phi \left(|_{-\frac{\pi}{2}}^0 - |_0^{\frac{\pi}{2}}\right) d\theta\\
&= -\frac{\ln^2 2}{2} \int_0^{2\pi} d\theta\\
&= \pi \ln^2 2
\end{align*}$$
