#+TITLE: Week 3.10 Math Homework
#+AUTHOR: 2024110144
#+LATEX_CLASS: article
#+LATEX_CLASS_OPTIONS: [a4paper,12pt]
#+LATEX_HEADER: \usepackage[margin=0.5in]{geometry}
#+OPTIONS: \n:t toc:nil num:nil date:nil

#+BEGIN_COMMENT
3.10 Thomas 14.2 35-40 odd
3.12 微积分学导论下 6.1 8 even 11 odd
3.14 Thomas 14.3 1-92 mod 6
     14.5 1-40 mod 5
#+END_COMMENT

* 3.10
# at what points in space are the functions in 35-40 continuous?
** 35
*** a $f(x,y,z)=x^2+y^2-2z^2$
since this function is polynomail, it is continuous everywhere in the real number space
*** b $f(x,y,z)=\sqrt{x^2+y^2-1}$
we need $x^2+y^2-1\geq 0$
then since $x, y, z$ for $x^2+y^2-1$ is continuous
we know that all points that satisfy $x^2+y^2\geq 1$ are continuous
** 37
*** a $h(x,y,z)=xy\sin\frac{1}{z}$
$z\neq 0$, no restriction for xy
so it is continuous for all $(x,y,z)$ above/below plane $xOy$ respectively
*** b $h(x,y,z)=\frac{1}{x^2+z^2-1}$
it is continuous for all $(x,y,z), x^2+z^2\neq 1$
in other words, it is continuous outside and inside assert $x^2+z^2=1$ separately.
** 39
*** a $h(x,y,z)=\sqrt{4-x^2-y^2-z^2}$
it is continuous for all the points inside sphere $x^2+y^2+z^2=4$.
*** b $h(x,y,z)=\frac{1}{4-\sqrt{x^2+y^2+z^2-9}}$
first, $x^2+y^2+z^2\geq 9$
second, $x^2+y^2+z^2\neq 25$
so it is continuous for
- points outside sphere $x^2+y^2+z^2=9$ but inside sphere $x^2+y^2+z^2=25$
- points outside sphere $x^2+y^2+z^2=25$
respectively

* 3.12
** 8
# 判断下列极限是否存在，若存在，求出其极限。
*** 2
$\lim_{\begin{align*} x &\rightarrow 0\\ y &\rightarrow 0\end{align*}} \frac{\sin xy}{x}$
yes, and it is $0$.
we can see so by multiplying $y$ and taking $\frac{\sin xy}{xy}$ as $1$.
*** 4
$\lim_{\begin{align*} x &\rightarrow \infty\\ y &\rightarrow a\end{align*}} \left(1+\frac{1}{x}\right)^{\frac{x^2}{x+y}}$
Using Taylor Expansion, we know when $x\rightarrow \infty$,
there is $\left(1+\frac{1}{x}\right)\rightarrow \frac{1}{x}$.
$\lim_{\begin{align*} x &\rightarrow \infty\\ y &\rightarrow a\end{align*}} e^{\frac{x^2}{x+y}\ln\left(1+\frac{1}{x}\right)}$
so the limit equals to that of $e^{\frac{x}{x+y}}$
the answer is $e$
*** 6
$\lim_{\begin{align*} x &\rightarrow \infty\\ y &\rightarrow \infty\end{align*}} \frac{x^2+y^2}{x^4+y^4}$
it is obviously $0$ no matter the equation we choose to describe the relationship between $x,y$
*** 8
$\lim_{\begin{align*} x &\rightarrow 1\\ y &\rightarrow 0\end{align*}} \frac{\ln \left(x+e^y\right)}{\sqrt{x^2+y^2}}$
when they approach their limits
the dividend would be $\ln 2$ and the dividor would be $1$
so the answer is $\ln 2$
*** 10
$\lim_{\begin{align*} x &\rightarrow 0\\ y &\rightarrow 0\end{align*}} \frac{\sqrt{xy+1}-1}{x+y}$
using $x+y\geq 2\sqrt{xy}$ we know the limit would not be greater than that of $\frac{\sqrt{xy+1}-1}{2\sqrt{xy}}$
which equals to that of $\frac{\sqrt{xy}}{2+2\sqrt{xy+1}}$
giving the upper bond $0$ for the limit
by the other hand, it is obvious that the limit would not be negative
so the answer is exactly $0$, ultilizing the sandwich law
*** 12
$\lim_{\begin{align*} x &\rightarrow 0\\ y &\rightarrow 0\end{align*}} (1+xy)^{\frac{1}{x+y}}$
the limit is equal to that of $e^{\frac{1}{x+y} \ln (1+xy)}$
where $\ln (1+xy)$ can be substituded by $xy$
examing the $\frac{xy}{x+y}$ which at last approaches $0$
giving us the answer of $1$
** 11
# 研究下列函数的连续性。
*** 1
$$f(x,y)=\left\{\begin{align*} & \frac{xy}{x+y}, & x\neq y\\
& 0, & x=y \end{align*}\right .$$;
for points not in $x=y$
they are continuous in groups separated by $x+y=0$
for points in $x=y$
they are of course continuous since they are all 0
for other situation
we have to check if points in $x=y$ is continuous with nearby points
which means $f(m,m)=\lim_{\begin{align*} x &\rightarrow m\\ y &\rightarrow m \end{align*}} f(x,y)$
which further indicates $\lim_{\begin{align*} x &\rightarrow m\\ y &\rightarrow m \end{align*}} f(x,y) = 0$
which is not correct when $m\neq 0$
just assign $y=kx$
*** 3
$$f(x,y)=\left\{\begin{align*} & \frac{x^2 y}{x^2+y^2}, & (x,y)\neq (0,0)\\
& 0, & (x,y)=(0,0) \end{align*}\right .$$;
it is continuous obviously for points other than $(0,0)$
then for the situation near $(0,0)$
since the function do approaches $0$ when it approaches $(0,0)$
we can see that by assigning $y=kx$
the function is continuous anywhere

* 3.14
** 14.3
*** 6
$f(x,y)=(2x-3y)^3$
\begin{align*}
\frac{\delta f}{\delta x} &= 6(2x-3y)^2\\
\frac{\delta f}{\delta y} &= -9(2x-3y)^2
\end{align*}
*** 12
$f(x,y)=\tan^{-1} \frac{y}{x}$
we know that the derivation of $\tan^{-1} u$ is $\frac{1}{1+u^2}$
\begin{align*}
\frac{\delta f}{\delta x} &= -\frac{y}{x^2+y^2}\\
\frac{\delta f}{\delta y} &= \frac{x}{x^2+y^2}
\end{align*}
*** 18
$f(x,y)=\cos^2 (3x-y^2)$
\begin{align*}
\frac{\delta f}{\delta x} &= -3 \sin (6x-2y^2)\\
\frac{\delta f}{\delta y} &= 2y \sin (6x-2y^2)
\end{align*}
*** 24
$f(x,y,z)=xy+xz+yz$
\begin{align*}
f_x &= y+z\\
f_y &= x+z\\
f_z &= x+y
\end{align*}
*** 30
$f(x,y,z)=yz+\ln (xy)$
\begin{align*}
f_x &= \frac{1}{x}\\
f_y &= z+\frac{1}{y}\\
f_z &= y
\end{align*}
*** 36
$g(u,v)=v^2 e^{\frac{2u}{v}}$
\begin{align*}
g_u &= 2v e^{\frac{2u}{v}}\\
g_v &= 2(v-u) e^{\frac{2u}{v}}
\end{align*}
*** 42
$f(x,y)=\sin xy$
\begin{align*}
f_{x^2} &= -y^2 \sin xy\\
f_{xy} &= \cos xy - xy \sin xy\\
f_{yx} &= \cos xy - xy \sin xy\\
f_{y^2} &= -x^2 \sin xy
\end{align*}
*** 48
$w=y e^{x^2-y}$
\begin{align*}
w_{x^2} &= 2y(1+2x^2) e^{x^2-y}\\
w_{xy} &= 2x(1-y) e^{x^2-y}\\
w_{yx} &= 2x(1-y) e^{x^2-y}\\
w_{y^2} &= (y-2) e^{x^2-y}
\end{align*}
*** 54
$w=x\sin y+y\sin x+xy$
\begin{align*}
w_x &= \sin y + y\cos x + y\\
w_y &= \sin x + x\cos y + x\\
w_{xy} &= \cos y + \cos x + 1\\
w_{yx} &= \cos y + \cos x + 1
\end{align*}
so that they are indeed equal
*** 60
$$f(x,y)=\left\{\begin{align*} & \frac{\sin (x^3+y^4)}{x^2+y^2}, & (x,y) \neq (0,0)\\
& 0, & (x,y) = (0,0) \end{align*}\right .$$
the one associated with $x$ is equal to $\lim_{h\rightarrow 0} \frac{f(h,0)-f(0,0)}{h-0}$
which evaluates to $0$
the counterpart about $y$ has the same output
so the partial derivatives there are both $0$
*** 66
at $(1,-1,-3)$
$$\frac{\delta x}{\delta z} = \lim_{h\rightarrow 0} \frac{f(1,-1,-3+h)-f(1,-1,-3)}{h}$$
gives $\frac{1}{6}$
just differentiate both sides with respect to $z$ then pass the point in
*** 72 WFL
$$f(x,y)=\left\{\begin{align*} & xy\frac{x^2-y^2}{x^2+y^2}, & (x,y)\neq 0,\\
& 0, & (x,y)=0.\end{align*}\right .$$
**** a
$$\begin{align*}
\frac{\delta f}{\delta y}(x,0) &= \lim_{h\rightarrow 0} \frac{f(x,h)-f(x,0)}{h}\\
&= \lim_{h\rightarrow 0} \frac{f(x,h)}{h}\\
&= \lim_{h\rightarrow 0} x \cdot \frac{x^2-h^2}{x^2+h^2}\\
&= x
\end{align*}$$
$$\begin{align*}
\frac{\delta f}{\delta x}(0,y) &= \lim_{h\rightarrow 0} \frac{f(h,y)-f(0,y)}{h}\\
&= \lim_{h\rightarrow 0} \frac{f(h,y)}{h}\\
&= \lim_{h\rightarrow 0} y \cdot \frac{h^2-y^2}{h^2+y^2}\\
&= -y
\end{align*}$$

**** b

from a we can see one is $1$ and the other is $-1$
they are not equal

*** 78
$f(x,y)=\tan^{-1}\frac{x}{y}$
the once partials are $\frac{y}{x^2+y^2}$ and $\frac{-x}{x^2+y^2}$ respectively
the second is $\pm \frac{2xy}{x^2+y^2}$
which add up to $0$, satisfying the Laplace equation

*** 84
$w=\ln (2x+2ct)$
one partial for $t$ is $\frac{c}{x+ct}$
for $x$ is $\frac{1}{x+ct}$
the second would be $\frac{-c^2}{(x+ct)^2}$ and $\frac{-1}{(x+ct)^2}$ respectively
after rising the latter one with $c^2$
it is obvious that the wave equation is satisfied

*** 90
$u(x,t)=\sin(\alpha x)\cdot e^{-\beta t}$
$\frac{\delta u}{\delta t} = -\beta \sin (\alpha x) \cdot e^{-\beta t}$
$\frac{\delta^2 u}{\delta x^2} = -\alpha^2 \sin(\alpha x)\cdot e^{-\beta t}$
we need $\beta=\alpha^2$ for this to be a solution

** 14.5

*** 5
$f(x,y)=\sqrt{2x+3y}$ at $(-1,2)$
$$\begin{align*}
f_x &= (2x+3y)^{-\frac{1}{2}}\\
f_y &= \frac{3}{2} (2x+3y)^{-\frac{1}{2}}
\end{align*}$$
assign $(-1,2)$ in the partial derivatives
we have $\frac{1}{2}$ and $\frac{3}{4}$ respectively
so the gradient is $\left(\frac{1}{2},\frac{3}{4}\right)$
#+begin_src gnuplot :file Thomas-14.5-5.png :exports both
  set term png size 300,300
  set xrange [-3:3]
  set yrange [-1:5]
  set xlabel "X"
  set ylabel "Y"
  set title "Thomas-14.5-5"

  f(x, y) = sqrt(2*x + 3*y)

  set contour
  set cntrparam levels discrete 2
  set view 0, 90
  splot f(x, y) with lines title "Level Curve: f(x, y) = 2"

  set arrow from -1, 2 to -1 + 0.5/1.414, 2 + 0.75/1.414 nohead lw 2 lc rgb "red" title "Gradient Vector"

  set pointsize 2
  set style fill solid 1.0
  set object 1 circle at -1, 2 radius 0.1 fillcolor rgb "blue" behind

  replot
#+end_src

#+RESULTS:
[[file:Thomas-14.5-5.png]]

*** 10
$f(x,y,z)=e^{x+y} \cos z+(y+1) \sin^{-1} x$ at $(0,0,\frac{\pi}{6})$
just calculate the partial derivations for $x,y,z$ and assign the point to it
we have $(\frac{\sqrt{3}}{2}+1,\frac{\sqrt{3}}{2},-\frac{1}{2})$

*** 15
$f(x,y,z)=xy+yz+zx,P_0 (1,-1,2),\vec{u}=3\vec{i}+6\vec{j}-2\vec{k}$
the partial derivation is $y+z,x+z,z+y$ respectively
so the gradient at $P_0$ is $(1,3,0)$
we normalize $\vec{u}$ to get $(\frac{3\vec{i}}{7},\frac{6\vec{j}}{7},\frac{-2\vec{k}}{7})$
the we just need to dot multiply the gradient and normalized $\vec{u}$
the answer is $3$

*** 20
$f(x,y)=x^2 y + e^{xy} \sin y, P_0=(1,0)$
the gradient is $(0,2)$
the normalized direction vector is $(0,1)$
so the desired derivative is $2$ and $-2$ for increase and decrease respectively
with direction of $(0,1)$ and $(0,-1)$ correspondingly

*** 25
$x^2+y^2=4,(\sqrt{2},\sqrt{2})$
the tangent line is $x+y=2\sqrt{2}$
#+begin_src gnuplot :file Thomas-14.5-25.png :exports both
     set term png size 300,300
     set title "Thomas-14.5-25"
     set xlabel "X"
     set ylabel "Y"
     set xrange [-3:3]
     set yrange [-3:3]
     f(x, y) = x**2 + y**2 - 4
     x0 = sqrt(2.0)
     y0 = sqrt(2.0)
     gradx = 2*sqrt(2.0)
     grady = 2*sqrt(2.0)
     tangent(x) = y0 + (grady/gradx) * (x-x0)

     splot f(x,y) title "circle",\
	   tangent(x) title "tangent",\
	   x0, y0 with points pt 7 lc rgb "red" title "Point (sqrt(2), sqrt(2))",\
	   x0 + gradx/2, y0 + grady/2 with vectors x0, y0 nohead lw 2 lc rgb "blue" title "∇f"
#+end_src

#+RESULTS:
[[file:Thomas-14.5-25.png]]

*** 30
$f(x,y)=\frac{x-y}{x+y}$
it asks for $\vec{u}$ and the value of $D_u f\left(-\frac{1}{2},\frac{3}{2}\right)$
so that $D_u$
- a is largest
  we found that $D_u=3X_{\vec{u}}+Y_{\vec{u}}$
  so the answer is $(1,0),3$
- b is smallest
  $(-1,0),-3$
- c $=0$
  $(0,-3)$
- d $=-2$
  $(-\frac{2}{3},1)$
- e $=1$
  $(0,1)$

*** 35
# The derivative of f(x,y) at P_0(1,2) in the direction of i+j is 2\sqrt{2} and in the direction of -2j is -3. what is the derivative of f in the direction  of -i-2j? give reasons for your answer.
from the first two messages we can get $\nabla f = (1,3)$
which we can just dot multiply with normalized vector
to get the final answer $-\frac{7\sqrt{5}}{5}$

*** 40
well, we have $\nabla (fg) = g \nabla f + f \nabla g$
and a similar chain rule
not quite clear what does this quetion want
