#+TITLE: Week 5.19 Math Homework
#+AUTHOR: 2024110144 陈有骏
#+LATEX_COMPILER: xelatex
#+LATEX_CLASS: article
#+LATEX_CLASS_OPTIONS: [a4paper,10pt]
#+LATEX_HEADER: \usepackage[margin=0.5in]{geometry}
#+LATEX_HEADER: \usepackage{xeCJK}
#+LATEX_HEADER: \usepackage{fontspec}
#+LATEX_HEADER: \setCJKmainfont{WenQuanYi Zen Hei}
#+OPTIONS: \n:t toc:nil num:nil date:nil

#+begin_comment
5.19 Thomas 16.8 1-32 mod 4
left: 4 16 20 24 28 32
5.21 导论 7.7 二三四五六和二十一中奇数题
5.23 Thomas 8.8 1-64 mod 4 无穷积分
#+end_comment

* 5.19
** 4
** 8
$$F=x^2\vec{i}+xz\vec{j}+3z\vec{k}$$
$$D:\,x^2+y^2+z^2\leq 4$$
$$\begin{align*}
\iint_S F dS
&= \iiint_V \nabla \cdot F dV\\
&= \iiint_V (2x+0+3) dV\\
&= \iiint_V (2x+3) dV\\
&= \iiint_V (2z+3) dV\\
&= \int_{-2}^{2}\int_{-\sqrt{4-z^2}}^{\sqrt{4-z^2}}\int_0^{2\pi} (2z+3) r d\theta dr dz\\
&= 2\pi \int_{-2}^{2}\int_{-\sqrt{4-z^2}}^{\sqrt{4-z^2}}(2z+3) rdr dz\\
&= 2\pi \int_{-2}^{2} 0 \cdot (2z+3) dz\\
&= 0
\end{align*}$$
** 12
$$F=x^3\vec{i}+y^3\vec{j}+z^3\vec{k}$$
$$D:\,x^2+y^2+z^2\leq a^2$$
$$\nabla \cdot F = 3(x^2+y^2+z^2)$$
$$\begin{align*}
\iint_S FdS
&= \iiint_V \nabla \cdot F dV\\
&= \iiint_V 3(x^2+y^2+z^2) dV\\
&= 3\iiint_V (x^2+y^2+z^2) dV\\
&= 3\iiint_V \rho^4\sin\phi dV\\
&= 3\int_0^{2\pi} \int_0^{\pi} \int_0^a \rho^4\sin\phi d\rho d\phi d\theta\\
&= \frac{3}{5} \int_0^{2\pi} \int_0^{\pi} a^5\sin\phi d\phi d\theta\\
&= \frac{3a^5}{5} \int_0^{2\pi} \int_0^{\pi} \sin\phi d\phi d\theta\\
&= \frac{3a^5}{5} \int_0^{2\pi} -\cos\phi |_0^{\pi} d\theta\\
&= \frac{3a^5}{5} \int_0^{2\pi} 2 d\theta\\
&= \frac{6a^5}{5} \int_0^{2\pi} d\theta\\
&= \frac{12a^5\pi}{5}
\end{align*}$$
** 16
$$F=\ln (x^2+y^2)\vec{i}-\left(\frac{2z}{x}\tan^{-1}\frac{y}{x}\right)\vec{j}+z\sqrt{x^2+y^2}\vec{k}$$
$$D:\,1\leq x^2+y^2 \leq 2, -1\leq z \leq 2$$
$$\nabla \cdot F = \frac{2x}{x^2+y^2} - \frac{2z}{x^2+y^2} + \sqrt{x^2+y^2}$$
$$\begin{align*}
\iint_S FdS
&= \iiint_V \nabla \cdot F dV\\
&= \iiint_V \frac{2x-2z}{x^2+y^2} + \sqrt{x^2+y^2} dV\\
&= \int_0^{2\pi} \int_{-1}^2 \int_1^{\sqrt{2}} \left(2\cos \theta + r - \frac{2z}{r}\right) rdr dz d\theta\\
&= \int_0^{2\pi} \int_{-1}^2 \int_1^{\sqrt{2}} \left(r - \frac{2z}{r}\right) rdr dz d\theta\\
&= \int_0^{2\pi} \int_{-1}^2 \int_1^{\sqrt{2}} \left(r - \frac{2z}{r}\right) rdr dz d\theta\\
&= -3\pi (\sqrt{2}-1) + 2\pi(2\sqrt{2}-1)\\
&= \pi \sqrt{2} + \pi
\end{align*}$$
** 20
** 24
** 28
** 32

* 5.21

* 5.23
** 12
suppose $a>2$
$$\begin{align*}
\int_2^{\infty} \frac{2dt}{t^2-1}
&= \lim_{a\to \infty} \int_2^a \frac{2dt}{t^2-1}\\
&= \lim_{a\to \infty} \int_2^a \frac{2}{t^2-1} dt\\
&= \lim_{a\to \infty} \int_2^a \frac{1}{t-1}-\frac{1}{t+1} dt\\
&= \lim_{a\to \infty} (\int_2^a \frac{1}{t-1} dt - \int_2^a \frac{1}{t+1} dt)\\
&= \lim_{a\to \infty} (\int_1^{a-1} \frac{1}{t} dt - \int_3^{a+1} \frac{1}{t} dt)\\
&= \lim_{a\to \infty} (\ln t |_1^{a-1} - \ln t |_3^{a+1})\\
&= \lim_{a\to \infty} (\ln (a-1) - \ln (a+1) + \ln 3)\\
&= \lim_{a\to \infty} (\ln \frac{a-1}{a+1} + \ln 3)\\
&= \ln 3
\end{align*}$$
** 20
$$\int_0^{\infty} \frac{16\tan^{-1} x}{1+x^2} dx$$
suppose $a>0$
then
$$\begin{align*}
\int_0^{\infty} \frac{16\tan^{-1} x}{1+x^2} dx
&= \lim_{a\to \infty} \int_0^a \frac{16\tan^{-1} x}{1+x^2} dx\\
&= \lim_{a\to \infty} 16 \int_0^a \frac{\tan^{-1} x}{1+x^2} dx\\
&= \lim_{a\to \infty} 16 \int_0^a \frac{\tan^{-1} x}{1+x^2} dx
\end{align*}$$
Can't integrate this
** 24
$$\int_{-\infty}^{\infty} 2xe^{-x^2} dx$$
we suppose $a<0,b>0$
then
$$\begin{align*}
\int_{-\infty}^{\infty} 2xe^{-x^2} dx
&= \lim_{a\to -\infty, b\to \infty} \int_a^0 2xe^{-x^2} dx + \int_0^b 2xe^{-x^2} dx\\
&= \lim_{a\to -\infty, b\to \infty} \int_a^0 e^{-x^2} dx^2 + \int_0^b e^{-x^2} dx^2\\
&= \lim_{a\to -\infty, b\to \infty} \int_{a^2}^0 e^{-x} dx + \int_0^{b^2} e^{-x} dx\\
&= \lim_{a\to -\infty, b\to \infty} \int_0^{a^2} e^x dx - \int_0^{b^2} e^x dx\\
&= \lim_{a\to -\infty, b\to \infty} e^{a^2} - e^{b^2}\\
&= \lim_{a\to -\infty, b\to \infty} e^{a^2} - e^{b^2}
&= 0
\end{align*}$$
well, it is reasonable since the function is odd

** 48
$$\int_4^{\infty} \frac{dx}{\sqrt{x}-1}$$
suppose $a>4$,
we have
$$\begin{align*}
\int_4^{\infty} \frac{dx}{\sqrt{x}-1}
&= \lim_{a\to\infty} \int_4^a \frac{dx}{\sqrt{x}-1}\\
&= \lim_{a\to\infty} \int_2^{\sqrt{a}} \frac{2ydy}{y-1}\\
&= \lim_{a\to\infty} \int_2^{\sqrt{a}} \frac{2y}{y-1} dy\\
&= \lim_{a\to\infty} \int_2^{\sqrt{a}} 2+\frac{2}{y-1} dy\\
&= \lim_{a\to\infty} \int_2^a 2+\frac{2}{y-1} dy\\
&= \lim_{a\to\infty} (\int_2^a 2dy + \int_2^a \frac{2}{y-1} dy)\\
&= \lim_{a\to\infty} (2a-4 + 2\int_2^a \frac{1}{y-1} dy)\\
&= \lim_{a\to\infty} (2a-4 + 2\int_1^{a-1} \frac{1}{z} dz)\\
&= \lim_{a\to\infty} (2a-4 + 2\int_1^a \frac{1}{z} dz)\\
&= \lim_{a\to\infty} (2a-4 + 2\ln z |_1^a)\\
&= \lim_{a\to\infty} (2a-4 + 2\ln a - 0)\\
&= \lim_{a\to\infty} (2a-4+2\ln a)\\
&= \infty
\end{align*}$$

** 52
$$\int_2^{\infty} \frac{dx}{\sqrt{x^2-1}}$$
suppose $a>2$
we have
$$\begin{align*}
\int_2^{\infty} \frac{dx}{\sqrt{x^2-1}}
&= \lim_{a\to\infty} \int_2^a \frac{dx}{\sqrt{x^2-1}}\\
&= \lim_{a\to\infty} \int_{\sec^{-1} 2}^{\sec^{-1} a} \sec\theta d\theta\\
&= \lim_{a\to\infty} \ln (\sec\theta+\tan\theta) |_{\sec^{-1} 2}^{\sec^{-1} a}\\
&= \lim_{a\to\infty} \ln \frac{\left| a+\sqrt{a^2-1} \right|}{2+\sqrt{3}}\\
&= \infty
\end{align*}$$

** 56
$$\int_{\pi}^{\infty} \frac{1+\sin x}{x^2} dx$$
suppose $a>\pi$
then
$$\begin{align*}
\int_{\pi}^{\infty} \frac{1+\sin x}{x^2} dx
&= \lim_{a\to\infty} \int_{\pi}^a \frac{1+\sin x}{x^2} dx\\
&= \lim_{a\to\infty} (\int_{\pi}^a \frac{1}{x^2} dx + \int_{\pi}^a \frac{\sin x}{x^2} dx)\\
&= \lim_{a\to\infty} (-\frac{1}{x} |_{\pi}^a + \int_{\pi}^a \frac{\sin x}{x^2} dx)\\
&= \lim_{a\to\infty} (\frac{1}{\pi} - \frac{1}{a} + \int_{\pi}^a \frac{\sin x}{x^2} dx)\\
&= \frac{1}{\pi} + \lim_{a\to\infty} (- \frac{1}{a} + \int_{\pi}^a \frac{\sin x}{x^2} dx)\\
&= \frac{1}{\pi} + \lim_{a\to\infty} (\int_{\pi}^a \frac{\sin x}{x^2} dx)
\end{align*}$$
since the latter has $|\frac{\sin x}{x^2}|\leq |\frac{1}{x^2}|$
and we know $\frac{1}{\pi^2}$
integrating this outputs $\frac{1}{\pi}$
which means the answer is a finite constant
it is just I failed to work it out

** 60
$$\int_{e^e}^{\infty} \ln \ln x dx$$
suppose $a>e^e$
then
$$\begin{align*}
\int_{e^e}^{\infty} \frac{1+\sin x}{x^2} dx
&= \lim_{a\to\infty} \int_{e^e}^a \ln \ln x dx\\
&= \lim_{a\to\infty} (x\ln \ln x - \int \frac{1}{\ln x} dx) |_{e^e}^a\\
&= \lim_{a\to\infty} a - e^e - \int_{e^e}^a \frac{1}{\ln x} dx\\
&= \infty
\end{align*}$$

** 64
$$\int_{-\infty}^{\infty} \frac{dx}{e^x+e^{-x}}$$
suppose $a<0,b>0$
then
$$\begin{align*}
\int_{-\infty}^{\infty} \frac{dx}{e^x+e^{-x}}
&= \lim_{a\to -\infty, b\to \infty} (\int_a^0 \frac{dx}{e^x+e^{-x}} + \int_0^b \frac{dx}{e^x+e^{-x}})\\
&= \frac{1}{2} (\frac{\pi}{2}+\frac{\pi}{2})\\
&= \frac{\pi}{2}
\end{align*}$$
