#+TITLE: Week 10.20 Math Homework
#+AUTHOR: 2024110144 陈有骏
#+LATEX_COMPILER: xelatex
#+LATEX_CLASS: article
#+LATEX_CLASS_OPTIONS: [a4paper,10pt]
#+LATEX_HEADER: \usepackage[margin=0.5in]{geometry}
#+LATEX_HEADER: \usepackage{xeCJK}
#+LATEX_HEADER: \usepackage{fontspec}
#+LATEX_HEADER: \usepackage{amsmath}
#+LATEX_HEADER: \setCJKmainfont{WenQuanYi Zen Hei}
#+OPTIONS: \n:t toc:nil num:nil date:nil

#+begin_comment
3.2 31-38 mod 2 (P133)
3.3 25-36 mod 3 (P139)
3.4 30-34 mod 2 (P147)
3.5 1-30 mod 6 (P155)
3.6 1-26 mod 5 (P160)
#+end_comment

(repeated questions skipped)

* 3.2
** 32
$P(x)y''+Q(x)y'+R(x)y=0$
$(P(x)y')'+(f(x)y)'=0$
$P''(x)-Q'(x)+R(x)=0$

$y''+xy'+y=0$
$P(x)=1, Q(x)=x, R(x)=1$
$P''(x)-Q'(x)+R(x)=0-1+1=0$
so it is an exact equation
it can be written as $y''+(xy)'=0$
$y' = xy + C$
$y' - xy = C$
$(xy)' - 2(xy) = C$
suppose $u=xy$
so $u' - 2u = C$
$e^{-2x}u' - 2e^{-2x}u = C$
$e^{-2x}u = C_1x + C_2$
$u = C_1xe^{-2x} + C_2e^{-2x}$
$y = C_1e^{-2x} + C_2x^{-1}e^{-2x}$
** 34
$x^2y''+xy'-y=0, x>0$
$P(x)=x^2, Q(x)=x, R(x)=-1$
$P''(x)-Q'(x)+R(x)=2-1-1=0$
so it is an exact equation
it can be written as $(x^2y')'-(xy)'=0$
$x^2y'=xy + C$
$x^2y' - xy = C$
$xy' - y = \frac{1}{x}C$
$(xy)' - 2(xy) = \frac{1}{x}C$
$u'-2u=\frac{1}{x}C$
$e^{-2x}u=C_1\ln x + C_2$
$u = C_1\ln x\cdot e^{2x} + C_2\cdot e^{2x}$
$y = C_1\frac{\ln x}{x}\cdot e^{2x} + C_2\cdot x^{-1}\cdot e^{2x}$
** 36
$\mu(x)P(x)y'' + \mu(x)Q(x)y' + \mu(x)R(x)y=0$
$(\mu(x)P(x)y')' + (f(x)y)'=0$
$P\mu'' + (2P' - Q)\mu' + (P'' - Q' + R)\mu = 0$

$P(x)=x^2, Q(x)=x, R(x)=x^2-v^2$
$x^2\mu'' + 3x\mu' + (1 + x^2 - v^2)\mu = 0$
** 38
$P(x)=P(x), 2P'(x)-Q(x)=Q(x), P''(x)-Q'(x)+R(x) = R(x)$
so $P'(x)=Q(x), P''(x)=Q'(x)$
$36$ is not because $(x^2)'=2x\neq x$
$37$ indeed is because $1'=0$ with no second order differencials
* 3.3
** 27
let $x=\ln t$
$\begin{aligned}
\frac{dy}{dt} &= \frac{dy}{dx}\frac{dx}{dt}\\
&=\frac{dy}{tdx}
\end{aligned}$
$\begin{aligned}
\frac{d^2y}{dt^2}
&= \frac{1}{t}\frac{d^2y}{dxdt} - \frac{1}{t^2} \frac{dy}{dx}\\
&= \frac{1}{t^2}\frac{d^2y}{dx^2} - \frac{1}{t^2} \frac{dy}{dx}
\end{aligned}$

$t^2y'' + 4ty' + 2y = 0$
$\frac{d^2y}{dx^2} + 3\frac{dy}{dx} + 2y = 0$
$r^2+3r+2=0$
$(r+2)(r+1)=0$
$r=-2, -1$
$y=c_1e^{-2x}+c_2e^{-x}$
$W[e^{-2x}, e^{-x}] \neq 0$
$y=c_1e^{-2\ln t}+c_2e^{-\ln t}$
** 33
$x = \int (q(t))^{\frac{1}{2}} dt = \int e^{-\frac{t^2}{2}} dt = -\frac{1}{t}e^{-\frac{t^2}{2}} + C$
$y'' + ty' + e^{-t^2}y = 0, -\infty<t<\infty$
$\frac{dy}{dt} = (1+\frac{1}{t^2})e^{-\frac{t^2}{2}}\frac{dy}{dx}$
$\frac{d^2y}{dt^2} = (-t-\frac{1}{t}-\frac{2}{t^3})e^{-\frac{t^2}{2}}\frac{dy}{dx} + (1+\frac{1}{t^2})^2e^{-t^2} \frac{d^2y}{dx^2}$
$(1+\frac{1}{t^2})e^{-t^2} \frac{d^2y}{dx^2} - \frac{2}{t^3}e^{-\frac{t^2}{2}}\frac{dy}{dx} + e^{-t^2}y = 0$
tried many times but still not solving
** 36
since $q(t)<0$, it is not possible
* 3.4
** 32
let $x=\ln t$
$\begin{aligned}
\frac{dy}{dt} &= \frac{dy}{dx}\frac{dx}{dt}\\
&=\frac{dy}{tdx}
\end{aligned}$
$\begin{aligned}
\frac{d^2y}{dt^2}
&= \frac{1}{t}\frac{d^2y}{dxdt} - \frac{1}{t^2} \frac{dy}{dx}\\
&= \frac{1}{t^2}\frac{d^2y}{dx^2} - \frac{1}{t^2} \frac{dy}{dx}
\end{aligned}$

$\frac{d^2y}{dx^2} + \frac{dy}{dx} + 0.25y = 0$
$r^2+r+0.25=0$
$(r+0.5)^2=0$
$r=-0.5$
$y = c(1+x)e^{-0.5x}$
$y = c(1+\ln t)e^{-0.5\ln t}$
** 34
$4\frac{d^2y}{dx^2} - 12\frac{dy}{dx} + 9y = 0$
$(2r-3)^2=0
$r=\frac{3}{2}$
$y = c(1+x)e^{\frac{3}{2}x}$
$y = c(1+\ln t)e^{\frac{3}{2}\ln t}$
* 3.5
** 6
$y''+2y'+y=2e^{-t}$
*** first seek the particular solution $Y$
suppose $Y(t) = Ae^{-t}$
then $Ae^{-t} - 2Ae^{-t} + Ae^{-t} = 0\neq 2e^{-t}$
suppose $Y(t) = Ate^{-t}$
then $A(t-2)e^{-t} + 2A(1-t)e^{-t} + Ate^{-t} = 2e^{-t}$
so $At - 2A + 2A - 2At + At = 0\neq 2e^{-t}$
suppose $Y(t) = A(t)e^{-t}$
then $Y'(t) = (A(t)-A'(t))e^{-t}$ and $Y''(t) = (A(t) - 2A'(t) + A''(t))e^{-t}$
so $4A(t) - 4A'(t) + A''(t) = 2$
suppose $A(t)=a(t) + \frac{1}{2}$
then $4a(t) - 4a'(t) + a''(t) = 0$
so $r^2 - 4r + 4 = $
$r=2$
$a = c(1+t)e^{2t}$
so $A(t) = c(1+t)e^{2t} + \frac{1}{2}$
let $c = 1$
$Y = (1+t)e^t + \frac{1}{2}e^{-t}$
*** then we look for homogenious solution
for $y'' + 2y' + y = 0$
we know $r = -1$
so $y = c(1+t)e^{-t}$
*** combine the answers
we get $y = (c + \frac{1}{2} + ct)e^{-t} + (1+t)e^t$

** 12
$y'' + 4y = t^2 + 3e^t$
*** $t^2$
$y'' + 4y = t^2$
suppose $Y = at^2 + bt + c$
then $Y' = 2at + b$
$Y'' = 2a$
$2a + 4at^2 + 4bt + 4c = t^2$
so $Y = \frac{1}{4} t^2 - \frac{1}{8}$
*** $3e^t$
$y'' + 4y = 3e^t$
suppose $Y = Ae^t$
then $A + 4A = 3$, giving $A=\frac{3}{5}$
so $Y = \frac{3}{5}e^t$
*** $0$
$r^2 + 4 = 0$
$r = 2i$
$y = c(1+t)e^{2ti}$
$y = c(1+t)(\cos 2t + i\sin 2t)$
*** combine
$y = c(1+t)(\cos 2t + i\sin 2t) + \frac{1}{4} t^2 + \frac{3}{5}e^t - \frac{1}{8}$
** 18
$y'' + 2y' + 2y = 3e^{-t} + 2e^{-t}\cos t + 4e^{-t}t^2\sin t$
*** a
$Y = Ae^{-t} + (B\cos t + C\sin t)e^{-t} + ((Dt^2+Et+F)\cos t + (Gt^2 + Ht + I)\sin t)e^{-t}$
which is $Y = e^{-t}((A_0t^2 + A_1t + A_2)\cos t + (B_0t^2 + B_1t + B_2)\sin t + C)$
*** b
suppose $y_1(t) = y(t)$ and $y_2(t) = y_1'(t)$
as suggested by [[https://math.umd.edu/~petersd/460/html/ode45_demo2.html][this link]] on University of Maryland math page
and [[https://gistlib.com/matlab/solve-second-order-differential-equation-in-matlab][this link]] on gistlib
similar info can be found on MathWork's webpage
need initial condition, since $y_2'(0) + y_2(0) + y_1(0) = 5$
and we just need a particular solution, use $y_2(0) = 0, y_1(0) = 0$ 
we have $\begin{bmatrix} y_1' \\ y_2' \end{bmatrix} = \begin{bmatrix} y_2 \\ 3e^{-t} + 2e^{-t}\cos t + 4e^{-t}t^2\sin t - 2y_2 - 2y_1 \end{bmatrix}$
and $\begin{bmatrix} y_1(0) \\ y_2(0) \end{bmatrix} = \begin{bmatrix} 0 \\ 0 \end{bmatrix}$
now use octave (compatible with matlab by syntax) to plot a particular $y$ solution
#+begin_src octave :results file graphics :file 3.5-18-b.png :exports both
  f = @(t, y) [y(2); exp(-t)*(3 + 2*cos(t) + 4*realpow(t, 2)*sin(t)) - 2*y(2) - 2*y(1)];
  %% this is a vector function, y(2) means the second row, first element in matrix y
  t0 = 0; tn = 20; y0 = [0; 0];

  [ts, ys] = ode45(f, [t0, tn], y0); % use ode45 to solve IVP (1st O.D.E. only)

  figure(1, "visible", "off"); % walkaround from org doc, open an invisible window for plotting
  plot(ts, ys(:, 1), "blue"); % plot solution y(t)
  title("y(t) when y(0)=y'(0)=0");
  xlabel('t');
  ylabel('y');
  grid on;
  print -dpng 3.5-18-b.png; % mannually safe whatever on the window
  ans = "3.5-18-b.png";
#+end_src

#+RESULTS:
[[file:3.5-18-b.png]]

** 24
*** $y''+y=t$
for $y''+y=0$, we have $r=i$
so $y = c(1+t)e^{it}$
for $y''+y=t$, a particular solution,
we suppose $Y = At+B$
so $At+B=t$, indicating $A=1, B=0$
so $Y=t$
giving $y = c(1+t)(\cos t + i\sin t) + t$
apply initial conditions
we get $c = 0$
so $y = t$
*** $y'' + y = \pi e^{\pi - t}$
we know $y(\pi)=\pi, y'(\pi)=1$ as new initial values
suppose $Y = Ae^{\pi - t}$
we get $2A = \pi$
so $Y=\frac{\pi}{2} e^{\pi - t}$
$y = c(1+t)(\cos t + i\sin t) + \frac{\pi}{2} e^{\pi - t}$
considering $t=\pi$, we get $-c(1+\pi) = \frac{\pi}{2}$
so $c = -\frac{\pi}{2+2\pi}$
$y = -\frac{\pi}{2+2\pi}(1+t)(\cos t + i\sin t) + \frac{\pi}{2} e^{\pi - t}$
then use gnuplot to plot whole function
#+begin_src gnuplot :results file graphics :file 3.5-24.png :exports both
  set xlabel "t";
  unset ylabel;
  unset zlabel;
  set parametric;
  set view 60, 150, 1, 1;
  set urange [0:10];
  unset title;

  f(x) = (x <= pi) ? x : -pi/(2+2*pi)*(1+x)*exp(I*x)+pi/2*exp(pi-x);

  splot u, real(f(u)), real(-I*f(u)) notitle;
#+end_src

#+RESULTS:
[[file:3.5-24.png]]

** 30
$y''+2y'=(D^2+2D)y=3+4\sin(2t)$
$D^2+2D=D(D+2)$
so $r_1=0, r_2=-2$
let $u=(D+2)y$
don't understand the "D denotes differetiation with respect to t" statement
* 3.6
** 5
$y''+9y = 9\sec^2(3t), 0<t<\frac{\pi}{6}$
suppose $Y = A\sec (6t) + B\csc (6t)$
for $y'' + 9y = 0$
we know $r^2 + 9 = 0$
so $y = c(1+t)e^{3ti}$
where $y_1 = e^{3ti}, y_2 = te^{3ti}$
then $W[y_1, y_2] = e^{6ti}$
pick $t_0 = 0$
we have $Y = -e^{3ti}\int_0^t \frac{se^{3si}\cdot 9\sec^2(3s)}{e^{6si}} ds + te^{3ti} \int_0^t \frac{e^{3si}\cdot 9\sec^2(3s)}{3^{6si}} ds$
so the general solution is $y = c(1+t)e^{3ti} + -e^{3ti}\int_0^t \frac{se^{3si}\cdot 9\sec^2(3s)}{e^{6si}} ds + te^{3ti} \int_0^t \frac{e^{3si}\cdot 9\sec^2(3s)}{3^{6si}} ds$
** 10
$t^2y'' - 2y = 3t^2 - 1, t>0; y_1(t) = t^2, y_2(t) = t^{-1}$
for $y_1$, $2t^2 - 2t^2 = 0$
for $y_2$, $2t^2\cdot t^{-3} - 2t^{-1} = 0$
$W[y_1, y_2] = -3 \neq 0$
so they satisfy the corresponding homogenious equation
and constitutes a fundamental solution set
here $g(t) = 3t^2 - 1$
let $t_0 = 1$
we have
$\begin{aligned}
Y(t) &= \frac{t^2}{3}\int_{t_0}^t \frac{1}{s} (3s^2 - 1) ds - \frac{1}{3t} \int_{t_0}^t s^2(3s^2 - 1) ds\\
&= \frac{t^2}{3}\int_{t_0}^t (3s - \frac{1}{s}) ds - \frac{1}{3t} \int_{t_0}^t (3s^4 - s^2) ds\\
&= \frac{t^2}{3}(\frac{3}{2}s^2 - \ln s + C_1)|_{t_0}^t - \frac{1}{3t} (\frac{3}{5} s^5 - \frac{1}{3} s^2|_{t_0}^t\\
&= \frac{t^2}{3}(\frac{3}{2}(t^2-t_0^2) - \ln \frac{t}{t_0}) - \frac{1}{3t} (\frac{3}{5} (t^5-t_0^5) - \frac{1}{3} (t^2-t_0^2)\\
&= \frac{t^2}{2}(t^2-t_0^2) - \frac{t^2}{3}\ln \frac{t}{t_0} - \frac{1}{5t} (t^5-t_0^5) + \frac{1}{9t} (t^2-t_0^2)\\
&= \frac{t^2}{2}(t^2-1) - \frac{t^2}{3}\ln t - \frac{1}{5t} (t^5-1) + \frac{1}{9t} (t^2-1)
\end{aligned}$

** 15
$x^2y''+xy'+(x^2-\frac{1}{4})y = 3x^{\frac{3}{2}}\sin x, x>0; y_1(x)=x^{-\frac{1}{2}}\sin x, y_2(x) = x^{-\frac{1}{2}}\cos x$
let $t=\ln x$, $y' = \frac{1}{x}\frac{dy}{dt}$, $y'' = \frac{1}{x^2}\frac{d^2y}{dt^2} - \frac{1}{x^2} \frac{dy}{dt}$
so $\frac{d^2y}{dt^2} + (e^{2t}-\frac{1}{4})y = 3e^{\frac{3}{2}t}\sin e^t, t\in\mathbb{R}$
with shifted $y_1, y_2$
and $y_1(t) = e^{-\frac{1}{2}t}\sin e^t, y_2(t) = e^{-\frac{1}{2}t}\cos e^t$
apply $y_1$,
get $-\frac{1}{2}e^{-\frac{1}{2}t}\sin e^t + e^{\frac{1}{2}t}\cos e^t + (e^{2t}-\frac{1}{4})e^{-\frac{1}{2}t}\sin e^t$
not zero, not knowing where is wrong
** 20
question $16$ tells us $Y(t)= \int_{t_0}^t \frac{y_1(s)y_2(t)-y_2(s)y_1(t)}{y_1(s)y_2'(s)-y_1'(s)y_2(s)} g(s) ds$
for $y'' - 2\lambda y' + (\lambda^2+\mu^2) y = 0$
$y_1 = e^{(\lambda + \mu i)t}, y_2 = e^{(\lambda - \mu i)t}$
$y_1' = (\lambda + \mu i)e^{(\lambda + \mu i)t}, y_2' = (\lambda - \mu i)e^{(\lambda - \mu i)t}$
$Y(t) = \int_{t_0}^t \frac{e^{(\lambda + \mu i)s}e^{(\lambda - \mu i)t}-e^{(\lambda - \mu i)s}e^{(\lambda + \mu i)t}}{e^{(\lambda + \mu i)s}(\lambda - \mu i)e^{(\lambda - \mu i)s}-(\lambda + \mu i)e^{(\lambda + \mu i)s}e^{(\lambda - \mu i)s}} g(s) ds$
so $y = Ae^{(\lambda + \mu i)t} + Be^{(\lambda - \mu i)t} + \int_{t_0}^t \frac{e^{(\lambda + \mu i)s}e^{(\lambda - \mu i)t}-e^{(\lambda - \mu i)s}e^{(\lambda + \mu i)t}}{e^{(\lambda + \mu i)s}(\lambda - \mu i)e^{(\lambda - \mu i)s}-(\lambda + \mu i)e^{(\lambda + \mu i)s}e^{(\lambda - \mu i)s}} g(s) ds$
** 25
$t^2y'' + 7ty' + 5y = t, t>0; y_1(t) = \frac{1}{t}$
first change with $x=\ln t$, and switch $y, y_1$
so $y'' + 6y' + 5y = e^x, x\in\mathbb{R}; y_1(x) = e^{-x}$
suppose $y(x) = v(x)y_1(x)$
then $e^{-x}v'' + 4e^{-x}v' = e^{-x}$
so $v'' + 4v' = 1$
suppose $u(x) = v'(x) - \frac{1}{4}$
then $u' + 4u = 0$
so $e^{4x}u' + 4e^{4x}u = 0$
giving $e^{4x}u = C$
which means $u(x) = Ce^{-4x}$
then $v'(x) = Ce^{-4x} + \frac{1}{4}$
so $v(x) = Ae^{-4x} + \frac{1}{4}x + B$
then $y(x) = Ae^{-5x} + \frac{1}{4}xe^{-x} + Be^{-x}$
so the original $y(t) = \frac{A}{t^5} + \frac{\ln t}{4t} + \frac{B}{t}$
